Stage work porting TransTheory

examples/CCS/CCSScript.sml
@@ -1,14 +1,19 @@
-(*
- * Copyright 1991-1995  University of Cambridge (Author: Monica Nesi)
- * Copyright 2016-2017  University of Bologna, Italy (Author: Chun Tian)
- * Copyright 2018-2019  Fondazione Bruno Kessler, Italy (Author: Chun Tian)
- * Copyright 2023-2024  The Australian National University (Author: Chun Tian)
- *)
+(* ========================================================================== *)
+(* FILE          : CCSScript.sml                                              *)
+(* DESCRIPTION   : A formalization of the process algebra CCS in HOL          *)
+(*                                                                            *)
+(* COPYRIGHTS    : 1991-1995 University of Cambridge (Monica Nesi)            *)
+(*                 2016-2017 University of Bologna, Italy (Chun Tian)         *)
+(*                 2018-2019 Fondazione Bruno Kessler, Italy (Chun Tian)      *)
+(*                 2023-2024 Australian National University (Chun Tian)       *)
+(******************************************************************************)
 
 open HolKernel Parse boolLib bossLib;
 
 open pred_setTheory pred_setLib relationTheory optionTheory listTheory CCSLib
      rich_listTheory;
+
+open generic_termsTheory binderLib nomsetTheory nomdatatype;
 
 open LabelTheory;
 
@@ -16,56 +21,190 @@ val _ = new_theory "CCS";
 
 val set_ss = std_ss ++ PRED_SET_ss;
 
-(******************************************************************************)
-(*                                                                            *)
-(*             Syntax of pure CCS ('a, 'b) (general formalization)            *)
-(*                                                                            *)
-(******************************************************************************)
-
-(* Define the type of (pure) CCS agent expressions. *)
+(* The (equivalent) old way (no alpha conversion)
 Datatype: CCS = nil
-              | var 'a
-              | prefix ('b Action) CCS
+              | var string
+              | prefix ('a Action) CCS
               | sum CCS CCS
               | par CCS CCS
-              | restr (('b Label) set) CCS
-              | relab CCS ('b Relabeling)
-              | rec 'a CCS
+              | restr ('a Label set) CCS
+              | relab CCS ('a Relabeling)
+              | rec string CCS
 End
+ *)
+
+(* The new way based on "examples/lambda/basics/generic_termsTheory
+
+   NOTE: it defines “:'a CCS” where 'a is 'b of the old “:('a,'b) CCS”.
+ *)
+val tyname = "CCS";
+
+(* ‘GVAR s vv’ corresponds to ‘var 'a’ *)
+val vp = “(\n u:unit. n = 0)”;                                  (* 0. var *)
+
+val rep_t = “:unit + 'a Action + unit + unit + 'a Label set + 'a Relabeling + unit”;
+val d_tm = mk_var("d", rep_t);
+
+(* ‘GLAM v bv ts us’ corresponds to everything else. *)
+val lp =
+  “(\n ^d_tm tns uns.
+     n = 0 /\ ISL d /\ tns = [] ∧ uns = []  \/                  (* 1. nil *)
+     n = 0 /\ ISR d /\ ISL (OUTR d) /\ tns = [] /\ uns = [0] \/ (* 2. prefix *)
+     n = 0 /\ ISR d /\ ISR (OUTR d) /\ ISL (OUTR (OUTR d)) /\
+              tns = [] /\ uns = [0;0] \/                        (* 3. sum *)
+     n = 0 /\ ISR d /\ ISR (OUTR d) /\ ISR (OUTR (OUTR d)) /\
+              ISL (OUTR (OUTR (OUTR d))) /\
+              tns = [] /\ uns = [0;0] \/                        (* 4. par *)
+     n = 0 /\ ISR d /\ ISR (OUTR d) /\ ISR (OUTR (OUTR d)) /\
+              ISR (OUTR (OUTR (OUTR d))) /\
+              ISL (OUTR (OUTR (OUTR (OUTR d)))) /\
+              tns = [] ∧ uns = [0] \/                           (* 5. restr *)
+     n = 0 /\ ISR d /\ ISR (OUTR d) /\ ISR (OUTR (OUTR d)) /\
+              ISR (OUTR (OUTR (OUTR d))) /\
+              ISR (OUTR (OUTR (OUTR (OUTR d)))) /\
+              ISL (OUTR (OUTR (OUTR (OUTR (OUTR d))))) /\
+              tns = [] /\ uns = [0] \/                          (* 6. relab *)
+     n = 0 /\ ISR d /\ ISR (OUTR d) /\ ISR (OUTR (OUTR d)) /\
+              ISR (OUTR (OUTR (OUTR d))) /\
+              ISR (OUTR (OUTR (OUTR (OUTR d)))) /\
+              ISR (OUTR (OUTR (OUTR (OUTR (OUTR d))))) /\
+              tns = [0] ∧ uns = [])”;                           (* 7. rec *)
+
+val {term_ABS_pseudo11, term_REP_11, genind_term_REP, genind_exists,
+     termP, absrep_id, repabs_pseudo_id, term_REP_t, term_ABS_t, newty, ...} =
+    new_type_step1 tyname 0 {vp = vp, lp = lp};
+
+(* ----------------------------------------------------------------------
+    CCS operators
+   ---------------------------------------------------------------------- *)
+
+val [gvar,glam] = genind_rules |> SPEC_ALL |> CONJUNCTS;
+
+(* var *)
+val var_t = mk_var("var", “:string -> ^newty”)
+val var_def = new_definition(
+   "var_def", “^var_t s = ^term_ABS_t (GVAR s ())”);
+val var_termP = prove(
+  mk_comb(termP, var_def |> SPEC_ALL |> concl |> rhs |> rand),
+  srw_tac [][genind_rules]);
+val var_t = defined_const var_def;
+
+(* nil *)
+val nil_t = mk_var("nil", “:^newty”);
+val nil_def = new_definition(
+   "nil_def", “^nil_t = ^term_ABS_t (GLAM ARB (INL ()) [] [])”);
+val nil_termP = prove(“^termP (GLAM x (INL ()) [] [])”,
+    match_mp_tac glam >> srw_tac [][genind_term_REP]);
+val nil_t = defined_const nil_def;
+val nil_def' = prove(“^term_ABS_t (GLAM v (INL ()) [] []) = ^nil_t”,
+    srw_tac [][nil_def, GLAM_NIL_EQ, term_ABS_pseudo11, nil_termP]);
 
 val _ = TeX_notation { hol = "nil", TeX = ("\\ensuremath{\\mathbf{0}}", 1) };
 
+(* prefix *)
+val prefix_t = mk_var("prefix", “:'a Action -> ^newty -> ^newty”);
+val prefix_def = new_definition(
+   "prefix_def",
+  “^prefix_t u E = ^term_ABS_t (GLAM ARB (INR (INL u)) [] [^term_REP_t E])”);
+val prefix_termP = prove(
+  “^termP (GLAM x (INR (INL u)) [] [^term_REP_t E])”,
+    match_mp_tac glam >> srw_tac [][genind_term_REP]);
+val prefix_t = defined_const prefix_def;
+val prefix_def' = prove(
+  “^term_ABS_t (GLAM v (INR (INL u)) [] [^term_REP_t E]) = ^prefix_t u E”,
+    srw_tac [][prefix_def, GLAM_NIL_EQ, term_ABS_pseudo11, prefix_termP]);
+
+(* sum *)
+val sum_t = mk_var("sum", “:^newty -> ^newty -> ^newty”);
+val sum_def = new_definition(
+   "sum_def",
+  “^sum_t E1 E2 = ^term_ABS_t (GLAM ARB (INR (INR (INL ()))) []
+                                        [^term_REP_t E1; ^term_REP_t E2])”);
+val sum_termP = prove(
+  “^termP (GLAM x (INR (INR (INL ()))) [] [^term_REP_t E1; ^term_REP_t E2])”,
+    match_mp_tac glam >> srw_tac [][genind_term_REP]);
+val sum_t = defined_const sum_def;
+val sum_def' = prove(
+  “^term_ABS_t (GLAM v (INR (INR (INL ()))) []
+                       [^term_REP_t E1; ^term_REP_t E2]) = ^sum_t E1 E2”,
+    srw_tac [][sum_def, GLAM_NIL_EQ, term_ABS_pseudo11, sum_termP]);
+
+val _ = overload_on ("+", ``sum``); (* priority: 500 *)
+val _ = TeX_notation { hol = "+", TeX = ("\\ensuremath{+}", 1) };
+
+(* par *)
+val par_t = mk_var("par", “:^newty -> ^newty -> ^newty”);
+val par_def = new_definition(
+   "par_def",
+  “^par_t E1 E2 = ^term_ABS_t (GLAM ARB (INR (INR (INR (INL ())))) []
+                                        [^term_REP_t E1; ^term_REP_t E2])”);
+val par_termP = prove(
+  “^termP (GLAM x (INR (INR (INR (INL ())))) []
+                  [^term_REP_t E1; ^term_REP_t E2])”,
+    match_mp_tac glam >> srw_tac [][genind_term_REP]);
+val par_t = defined_const par_def;
+val par_def' = prove(
+  “^term_ABS_t (GLAM v (INR (INR (INR (INL ())))) []
+                       [^term_REP_t E1; ^term_REP_t E2]) = ^par_t E1 E2”,
+    srw_tac [][par_def, GLAM_NIL_EQ, term_ABS_pseudo11, par_termP]);
+
+val _ = set_mapped_fixity {fixity = Infixl 600,
+                           tok = "||", term_name = "par"};
+
+(* val _ = Unicode.unicode_version {u = UTF8.chr 0x007C, tmnm = "par"}; *)
+val _ = TeX_notation { hol = "||", TeX = ("\\ensuremath{\\mid}", 1) };
+
+(* restr *)
+val restr_t = mk_var("restr", “:'a Label set -> ^newty -> ^newty”);
+val restr_def = new_definition(
+   "restr_def",
+  “^restr_t L E = ^term_ABS_t (GLAM ARB (INR (INR (INR (INR (INL L))))) []
+                                        [^term_REP_t E])”);
+val restr_termP = prove(
+  “^termP (GLAM x (INR (INR (INR (INR (INL L))))) [] [^term_REP_t E])”,
+    match_mp_tac glam >> srw_tac [][genind_term_REP]);
+val restr_t = defined_const restr_def;
+val restr_def' = prove(
+  “^term_ABS_t (GLAM v (INR (INR (INR (INR (INL L))))) [] [^term_REP_t E]) =
+   ^restr_t L E”,
+    srw_tac [][restr_def, GLAM_NIL_EQ, term_ABS_pseudo11, restr_termP]);
+
 (* compact representation for single-action restriction *)
-val _ = overload_on ("nu", ``\(n :'b) P. restr {name n} P``);
-val _ = overload_on ("nu", ``restr``);
+val _ = overload_on("nu", “λ(n :'a) P. restr {name n} P”);
 
 val _ = add_rule {term_name = "nu", fixity = Closefix,
                   pp_elements = [TOK ("(" ^ UnicodeChars.nu), TM, TOK ")"],
                   paren_style = OnlyIfNecessary,
                   block_style = (AroundEachPhrase, (PP.INCONSISTENT, 2))};
 
-val _ = TeX_notation { hol = "(" ^ UnicodeChars.nu,
-                       TeX = ("\\ensuremath{(\\nu}", 1) };
+(* relab *)
+val relab_t = mk_var("relab", “:^newty -> 'a Relabeling -> ^newty”);
+val relab_def = new_definition(
+   "relab_def",
+  “^relab_t E rf =
+   ^term_ABS_t (GLAM ARB (INR (INR (INR (INR (INR (INL rf)))))) []
+                         [^term_REP_t E])”);
+val relab_termP = prove(
+  “^termP (GLAM x (INR (INR (INR (INR (INR (INL rf)))))) [] [^term_REP_t E])”,
+    match_mp_tac glam >> srw_tac [][genind_term_REP]);
+val relab_t = defined_const relab_def;
+val relab_def' = prove(
+  “^term_ABS_t (GLAM v (INR (INR (INR (INR (INR (INL rf)))))) []
+                       [^term_REP_t E]) =
+   ^relab_t E rf”,
+    srw_tac [][relab_def, GLAM_NIL_EQ, term_ABS_pseudo11, relab_termP]);
 
-(* TODO: send to HOL's boolTheory *)
-val _ = TeX_notation { hol = "(", TeX = ("\\ensuremath{(}", 1) };
-val _ = TeX_notation { hol = ")", TeX = ("\\ensuremath{)}", 1) };
-val _ = TeX_notation { hol = "=", TeX = ("\\ensuremath{=}", 1) };
-
-(* disabled: this "\mu" is conflict with the \mu action used in CCS papers
-val _ = overload_on ("mu", ``rec``);
-val _ = Unicode.unicode_version { u = UnicodeChars.mu, tmnm = "mu" };
-val _ = TeX_notation { hol = "mu", TeX = ("\\ensuremath{\\mu}", 1) };
- *)
-
-val _ = overload_on ("+", ``sum``); (* priority: 500 *)
-val _ = TeX_notation { hol = "+", TeX = ("\\ensuremath{+}", 1) };
-
-val _ = set_mapped_fixity { fixity = Infixl 600,
-                            tok = "||", term_name = "par" };
-
-(* val _ = Unicode.unicode_version {u = UTF8.chr 0x007C, tmnm = "par"}; *)
-val _ = TeX_notation { hol = "||", TeX = ("\\ensuremath{\\mid}", 1) };
+(* rec *)
+val rec_t = mk_var("rec", “:string -> ^newty -> ^newty”);
+val rec_def = new_definition(
+   "rec_def",
+  “^rec_t X E =
+   ^term_ABS_t (GLAM X (INR (INR (INR (INR (INR (INR ()))))))
+                       [^term_REP_t E] [])”);
+val rec_termP = prove(
+  “^termP (GLAM X (INR (INR (INR (INR (INR (INR ())))))) [^term_REP_t E] [])”,
+    match_mp_tac glam >> srw_tac [][genind_term_REP]);
+val rec_t = defined_const rec_def;
 
 val _ =
     add_rule { term_name = "prefix", fixity = Infixr 700,
@@ -75,43 +214,702 @@ val _ =
 
 val _ = TeX_notation { hol = "..", TeX = ("\\ensuremath{\\ldotp}", 1) };
 
-(* Define structural induction on CCS agent expressions. *)
-val CCS_induction = TypeBase.induction_of ``:('a, 'b) CCS``;
+(* ----------------------------------------------------------------------
+    tpm (permutation of CCS recursion variables)
+   ---------------------------------------------------------------------- *)
 
-(* The structural cases theorem for the type CCS. *)
-val CCS_cases = TypeBase.nchotomy_of ``:('a, 'b) CCS``;
+val cons_info =
+    [{con_termP = var_termP,    con_def = var_def},
+     {con_termP = nil_termP,    con_def = SYM nil_def'},
+     {con_termP = prefix_termP, con_def = SYM prefix_def'},
+     {con_termP = sum_termP,    con_def = SYM sum_def'},
+     {con_termP = par_termP,    con_def = SYM par_def'},
+     {con_termP = restr_termP,  con_def = SYM restr_def'},
+     {con_termP = relab_termP,  con_def = SYM relab_def'},
+     {con_termP = rec_termP,    con_def = rec_def}];
 
-(* Prove that the constructors of the type CCS are distinct. *)
-val CCS_distinct = TypeBase.distinct_of ``:('a, 'b) CCS``;
+val tpm_name_pfx = "t";
+val {tpm_thm, term_REP_tpm, t_pmact_t, tpm_t} =
+    define_permutation {name_pfx = tpm_name_pfx, name = tyname,
+                        term_REP_t = term_REP_t,
+                        term_ABS_t = term_ABS_t,
+                        absrep_id = absrep_id,
+                        repabs_pseudo_id = repabs_pseudo_id,
+                        cons_info = cons_info, newty = newty,
+                        genind_term_REP = genind_term_REP};
 
-(* size definition *)
-val (CCS_size_tm, CCS_size_def) = TypeBase.size_of ``:('a, 'b) CCS``;
+Theorem tpm_eqr:
+    t = tpm pi u <=> tpm (REVERSE pi) t = (u :'a CCS)
+Proof
+    METIS_TAC [pmact_inverse]
+QED
+
+Theorem tpm_eql:
+    tpm pi t = u <=> t = tpm (REVERSE pi) (u :'a CCS)
+Proof
+    simp[tpm_eqr]
+QED
+
+Theorem tpm_CONS :
+    tpm ((x,y)::pi) (t :'a CCS) = tpm [(x,y)] (tpm pi t)
+Proof
+  SRW_TAC [][GSYM pmact_decompose]
+QED
+
+(* ----------------------------------------------------------------------
+    support and FV
+   ---------------------------------------------------------------------- *)
+
+val term_REP_eqv = prove(
+   “support (fn_pmact ^t_pmact_t gt_pmact) ^term_REP_t {}”,
+    srw_tac [][support_def, fnpm_def, FUN_EQ_THM, term_REP_tpm, pmact_sing_inv]);
+
+val supp_term_REP = prove(
+   “supp (fn_pmact ^t_pmact_t gt_pmact) ^term_REP_t = {}”,
+    REWRITE_TAC [GSYM SUBSET_EMPTY]
+ >> MATCH_MP_TAC (GEN_ALL supp_smallest)
+ >> srw_tac [][term_REP_eqv]);
+
+val tpm_def' =
+    term_REP_tpm |> AP_TERM term_ABS_t |> PURE_REWRITE_RULE [absrep_id];
+
+val t = mk_var("t", newty);
+
+val supptpm_support = prove(
+   “support ^t_pmact_t ^t (supp gt_pmact (^term_REP_t ^t))”,
+    srw_tac [][support_def, tpm_def', supp_fresh, absrep_id]);
+
+val supptpm_apart = prove(
+   “x IN supp gt_pmact (^term_REP_t ^t) /\ y NOTIN supp gt_pmact (^term_REP_t ^t)
+    ==> ^tpm_t [(x,y)] ^t <> ^t”,
+    srw_tac [][tpm_def']
+ >> DISCH_THEN (MP_TAC o AP_TERM term_REP_t)
+ >> srw_tac [][repabs_pseudo_id, genind_gtpm_eqn, genind_term_REP, supp_apart]);
+
+val supp_tpm = prove(
+   “supp ^t_pmact_t ^t = supp gt_pmact (^term_REP_t ^t)”,
+    match_mp_tac (GEN_ALL supp_unique_apart)
+ >> srw_tac [][supptpm_support, supptpm_apart, FINITE_GFV]);
+
+val _ = overload_on ("FV", “supp ^t_pmact_t”);
+
+val _ = set_fixity "#" (Infix(NONASSOC, 450));
+val _ = overload_on ("#", “\X (E :'a CCS). X NOTIN FV E”);
+
+Theorem FINITE_FV[simp] :
+    FINITE (FV (t :'a CCS))
+Proof
+    srw_tac [][supp_tpm, FINITE_GFV]
+QED
+
+Theorem FV_EMPTY :
+    FV t = {} <=> !v. v NOTIN FV (t :'a CCS)
+Proof
+    SIMP_TAC (srw_ss()) [EXTENSION]
+QED
+
+fun supp_clause {con_termP, con_def} = let
+  val t = mk_comb(“supp ^t_pmact_t”, lhand (concl (SPEC_ALL con_def)))
+in
+  t |> REWRITE_CONV [supp_tpm, con_def, MATCH_MP repabs_pseudo_id con_termP,
+                     GFV_thm]
+    |> REWRITE_RULE [supp_listpm, EMPTY_DELETE, UNION_EMPTY]
+    |> REWRITE_RULE [GSYM supp_tpm]
+    |> GEN_ALL
+end
+
+Theorem FV_thm[simp] = LIST_CONJ (map supp_clause cons_info)
+
+val [FV_var, FV_nil, FV_prefix, FV_sum, FV_par,
+     FV_restr, FV_relab, FV_rec] =
+    map save_thm
+        (combine (["FV_var", "FV_nil", "FV_prefix", "FV_sum", "FV_par",
+                   "FV_restr", "FV_relab", "FV_rec"], CONJUNCTS FV_thm));
+
+(* |- !x t p. x IN FV (tpm p t) <=> lswapstr (REVERSE p) x IN FV t *)
+Theorem FV_tpm[simp] = “x IN FV (tpm p (t :'a CCS))”
+                       |> REWRITE_CONV [perm_supp, pmact_IN]
+                       |> GEN_ALL
+
+(* ----------------------------------------------------------------------
+    term induction
+   ---------------------------------------------------------------------- *)
+
+fun genit th = let
+  val (_, args) = strip_comb (concl th)
+  val (tm, x) = case args of [x,y] => (x,y) | _ => raise Fail "Bind"
+  val ty = type_of tm
+  val t = mk_var("t", ty)
+in
+  th |> INST [tm |-> t] |> GEN x |> GEN t
+end
+
+val LIST_REL_CONS1 = listTheory.LIST_REL_CONS1;
+val LIST_REL_NIL = listTheory.LIST_REL_NIL;
+
+val term_ind =
+    bvc_genind
+        |> INST_TYPE [alpha |-> rep_t, beta |-> “:unit”]
+        |> Q.INST [‘vp’ |-> ‘^vp’, ‘lp’ |-> ‘^lp’]
+        |> SIMP_RULE std_ss [LIST_REL_CONS1, RIGHT_AND_OVER_OR,
+                             LEFT_AND_OVER_OR, DISJ_IMP_THM, LIST_REL_NIL]
+        |> Q.SPECL [‘\n t0 x. Q t0 x’, ‘fv’]
+        |> UNDISCH |> Q.SPEC ‘0’ |> DISCH_ALL
+        |> SIMP_RULE (std_ss ++ DNF_ss)
+                     [sumTheory.FORALL_SUM, supp_listpm,
+                      IN_UNION, NOT_IN_EMPTY, oneTheory.FORALL_ONE,
+                      genind_exists, LIST_REL_CONS1, LIST_REL_NIL]
+        |> Q.INST [‘Q’ |-> ‘\t. P (^term_ABS_t t)’]
+        |> SIMP_RULE std_ss [GSYM var_def, GSYM nil_def, nil_def', prefix_def',
+                             sum_def', par_def', restr_def', relab_def',
+                             GSYM rec_def, absrep_id]
+        |> SIMP_RULE (srw_ss()) [GSYM supp_tpm]
+        |> elim_unnecessary_atoms {finite_fv = FINITE_FV}
+                                  [ASSUME “!x:'c. FINITE (fv x:string set)”]
+        |> SPEC_ALL |> UNDISCH
+        |> genit |> DISCH_ALL |> Q.GENL [‘P’, ‘fv’];
+
+fun mkX_ind th = th |> Q.SPECL [‘\t x. Q t’, ‘\x. X’]
+                    |> SIMP_RULE std_ss [] |> Q.GEN ‘X’
+                    |> Q.INST [‘Q’ |-> ‘P’] |> Q.GEN ‘P’;
+
+Theorem CCS_induction = mkX_ind term_ind
+
+Theorem simple_induction =
+    CCS_induction |> Q.SPECL [‘P’, ‘{}’]
+                  |> REWRITE_RULE [FINITE_EMPTY, NOT_IN_EMPTY]
+                  |> Q.GEN ‘P’
+
+Theorem rec_eq_thm =
+  “(rec u t1 = rec v t2 :'a CCS)”
+     |> SIMP_CONV (srw_ss()) [rec_def, rec_termP, term_ABS_pseudo11,
+                              GLAM_eq_thm, term_REP_11, GSYM term_REP_tpm,
+                              GSYM supp_tpm]
+     |> Q.GENL [‘u’, ‘v’, ‘t1’, ‘t2’]
+
+Theorem tpm_ALPHA :
+    v # (u :'a CCS) ==> rec x u = rec v (tpm [(v,x)] u)
+Proof
+    SRW_TAC [boolSimps.CONJ_ss][rec_eq_thm, pmact_flip_args]
+QED
+
+(* ----------------------------------------------------------------------
+    term recursion
+   ---------------------------------------------------------------------- *)
+
+val (_, repty) = dom_rng (type_of term_REP_t);
+val repty' = ty_antiq repty;
+
+val LENGTH_NIL' =
+    CONV_RULE (BINDER_CONV (LAND_CONV (REWR_CONV EQ_SYM_EQ)))
+              listTheory.LENGTH_NIL;
+
+val LENGTH1 = prove(
+   “(1 = LENGTH (l :'a list)) <=> ?e. l = [e]”,
+    Cases_on ‘l’ >> srw_tac [][listTheory.LENGTH_NIL]);
+
+val LENGTH2 = prove(
+   “(2 = LENGTH (l :'a list)) <=> ?a b. l = [a;b]”,
+    Cases_on ‘l’ >> srw_tac [][LENGTH1]);
+
+val termP_elim = prove(
+   “(!g. ^termP g ==> P g) <=> (!t. P (^term_REP_t t))”,
+    srw_tac [][EQ_IMP_THM] >- srw_tac [][genind_term_REP]
+ >> first_x_assum (qspec_then ‘^term_ABS_t g’ mp_tac)
+ >> srw_tac [][repabs_pseudo_id]);
+
+val termP_removal =
+    nomdatatype.termP_removal {
+      elimth = termP_elim, absrep_id = absrep_id,
+      tpm_def = AP_TERM term_ABS_t term_REP_tpm |> REWRITE_RULE [absrep_id],
+      termP = termP, repty = repty};
+
+val termP0 = prove(
+   “genind ^vp ^lp n t <=> ^termP t ∧ (n = 0)”,
+    EQ_TAC >> simp_tac (srw_ss()) [] >> strip_tac
+ >> qsuff_tac ‘n = 0’ >- (strip_tac >> srw_tac [][])
+ >> pop_assum mp_tac
+ >> Q.ISPEC_THEN ‘t’ STRUCT_CASES_TAC gterm_cases
+ >> srw_tac [][genind_GVAR, genind_GLAM_eqn]);
+
+(* “tvf :string -> 'q -> 'r” *)
+val tvf = “λ(s:string) (u:unit) (p:ρ). tvf s p : 'r”; (* var *)
+
+(* Type of constants occurring in tlf:
+
+   nil:    “tnf :'q -> 'r”
+   prefix: “tff :('q -> 'r) -> 'a Action -> 'a CCS -> 'q -> 'r”
+   sum:    “tsf :('q -> 'r) -> ('q -> 'r) -> 'a CCS -> 'a CCS -> 'q -> 'r”
+   par:    “tpf :('q -> 'r) -> ('q -> 'r) -> 'a CCS -> 'a CCS -> 'q -> 'r”
+   restr:  “trf :('q -> 'r) -> ('a Label -> bool) -> 'a CCS -> 'q -> 'r”
+   relab:  “tlf :('q -> 'r) -> 'a CCS -> 'a Relabeling -> 'q -> 'r”
+   rec:    “tcf :('q -> 'r) -> string -> 'a CCS -> 'q -> 'r”
+ *)
+val u_tm = mk_var("u", rep_t);
+val tlf =
+   “λ(v:string) ^u_tm (ds1:('q -> 'r) list) (ds2:('q -> 'r) list)
+                      (ts1:^repty' list) (ts2:^repty' list) (p :'q).
+       if ISL u then
+         tnf p :'r
+       else if ISL (OUTR u) then
+         tff (HD ds2) (OUTL (OUTR u)) (^term_ABS_t (HD ts2)) p :'r
+       else if ISL (OUTR (OUTR u)) then
+         tsf (HD ds2) (HD (TL ds2))
+             (^term_ABS_t (HD ts2)) (^term_ABS_t (HD (TL ts2))) p :'r
+       else if ISL (OUTR (OUTR (OUTR u))) then
+         tpf (HD ds2) (HD (TL ds2))
+             (^term_ABS_t (HD ts2)) (^term_ABS_t (HD (TL ts2))) p :'r
+       else if ISL (OUTR (OUTR (OUTR (OUTR u)))) then
+         trf (HD ds2) (OUTL (OUTR (OUTR (OUTR (OUTR u)))))
+             (^term_ABS_t (HD ts2)) p :'r
+       else if ISL (OUTR (OUTR (OUTR (OUTR (OUTR u))))) then
+         tlf (HD ds2) (^term_ABS_t (HD ts2))
+             (OUTL (OUTR (OUTR (OUTR (OUTR (OUTR u)))))) p :'r
+       else
+         tcf (HD ds1) v (^term_ABS_t (HD ts1)) p :'r”;
+
+Theorem parameter_tm_recursion =
+  parameter_gtm_recursion
+      |> INST_TYPE [alpha |-> rep_t, beta |-> “:unit”, gamma |-> “:'r”]
+      |> Q.INST [‘lf’ |-> ‘^tlf’, ‘vf’ |-> ‘^tvf’, ‘vp’ |-> ‘^vp’,
+                 ‘lp’ |-> ‘^lp’, ‘n’ |-> ‘0’]
+      |> SIMP_RULE (srw_ss()) [sumTheory.FORALL_SUM, FORALL_AND_THM,
+                               GSYM RIGHT_FORALL_IMP_THM, IMP_CONJ_THM,
+                               GSYM RIGHT_EXISTS_AND_THM,
+                               GSYM LEFT_EXISTS_AND_THM,
+                               GSYM LEFT_FORALL_IMP_THM,
+                               LIST_REL_CONS1, genind_GVAR,
+                               genind_GLAM_eqn, sidecond_def,
+                               NEWFCB_def, relsupp_def,
+                               LENGTH_NIL', LENGTH1, LENGTH2]
+      |> ONCE_REWRITE_RULE [termP0]
+      |> SIMP_RULE (srw_ss() ++ DNF_ss) [LENGTH1, LENGTH2,
+                                         listTheory.LENGTH_NIL]
+      |> CONV_RULE (DEPTH_CONV termP_removal)
+      |> SIMP_RULE (srw_ss()) [GSYM supp_tpm, SYM term_REP_tpm]
+      |> UNDISCH
+      |> rpt_hyp_dest_conj
+      |> lift_exfunction {repabs_pseudo_id = repabs_pseudo_id,
+                          term_REP_t = term_REP_t,
+                          cons_info = cons_info}
+      |> DISCH_ALL
+      |> elim_unnecessary_atoms {finite_fv = FINITE_FV}
+                                [ASSUME ``FINITE (A:string set)``,
+                                 ASSUME ``!p:ρ. FINITE (supp ppm p)``]
+      |> UNDISCH_ALL |> DISCH_ALL
+      |> REWRITE_RULE [AND_IMP_INTRO]
+      |> CONV_RULE (LAND_CONV (REWRITE_CONV [GSYM CONJ_ASSOC]))
+      |> Q.INST [‘tvf’ |-> ‘vr’, (* var *)
+                 ‘tnf’ |-> ‘nl’, (* nil *)
+                 ‘tff’ |-> ‘pf’, (* prefix *)
+                 ‘tsf’ |-> ‘sm’, (* sum *)
+                 ‘tpf’ |-> ‘pr’, (* par *)
+                 ‘trf’ |-> ‘rs’, (* restr *)
+                 ‘tlf’ |-> ‘rl’, (* relab *)
+                 ‘tcf’ |-> ‘re’, (* rec *)
+                 ‘dpm’ |-> ‘apm’]
+      |> CONV_RULE (REDEPTH_CONV sort_uvars)
+
+val FORALL_ONE = oneTheory.FORALL_ONE;
+val FORALL_ONE_FN = oneTheory.FORALL_ONE_FN;
+val EXISTS_ONE_FN = oneTheory.EXISTS_ONE_FN;
+
+Theorem tm_recursion =
+  parameter_tm_recursion
+      |> Q.INST_TYPE [‘:'q’ |-> ‘:unit’]
+      |> Q.INST [‘ppm’ |-> ‘discrete_pmact’,
+                  ‘vr’ |-> ‘\s u. vru s’,
+                  ‘nl’ |-> ‘\u. nlu’,
+                  ‘pf’ |-> ‘\r a t u. pfu (r()) a t’,
+                  ‘sm’ |-> ‘\r1 r2 t1 t2 u. smu (r1()) (r2()) t1 t2’,
+                  ‘pr’ |-> ‘\r1 r2 t1 t2 u. pru (r1()) (r2()) t1 t2’,
+                  ‘rs’ |-> ‘\r L t u. rsu (r()) L t’,
+                  ‘rl’ |-> ‘\r t rf u. rlu (r()) t rf’,
+                  ‘re’ |-> ‘\r v t u. reu (r()) v t’]
+      |> SIMP_RULE (srw_ss()) [FORALL_ONE, FORALL_ONE_FN, EXISTS_ONE_FN,
+                               fnpm_def]
+      |> SIMP_RULE (srw_ss() ++ CONJ_ss) [supp_unitfn]
+      |> Q.INST [‘vru’ |-> ‘vr’,
+                 ‘nlu’ |-> ‘nl’,
+                 ‘pfu’ |-> ‘pf’,
+                 ‘smu’ |-> ‘sm’,
+                 ‘pru’ |-> ‘pr’,
+                 ‘rsu’ |-> ‘rs’,
+                 ‘rlu’ |-> ‘rl’,
+                 ‘reu’ |-> ‘re’]
+
+(* ----------------------------------------------------------------------
+    cases, distinct and one-one theorems
+   ---------------------------------------------------------------------- *)
+
+Theorem CCS_cases :
+    !t. (t :'a CCS) = nil \/ (?a. t = var a) \/ (?u E. t = prefix u E) \/
+        (?E1 E2. t = sum E1 E2) \/ (?E1 E2. t = par E1 E2) \/
+        (?L E. t = restr L E) \/ (?E rf. t = relab E rf) \/
+         ?X E. t = rec X E
+Proof
+    HO_MATCH_MP_TAC simple_induction
+ >> SRW_TAC [][] (* 161 subgoals here *)
+ >> METIS_TAC []
+QED
+
+Theorem CCS_distinct[simp] :
+    (!X.     nil <> var X :'a CCS) /\
+    (!u E.   nil <> prefix u E :'a CCS) /\
+    (!E1 E2. nil <> E1 + E2 :'a CCS) /\
+    (!E1 E2. nil <> E1 || E2 :'a CCS) /\
+    (!L E.   nil <> restr L E :'a CCS) /\
+    (!E rf.  nil <> relab E rf :'a CCS) /\
+    (!X E.   nil <> rec X E :'a CCS) /\
+    (!X u E.   var X <> prefix u E :'a CCS) /\
+    (!X E1 E2. var X <> E1 + E2 :'a CCS) /\
+    (!X E1 E2. var X <> E1 || E2 :'a CCS) /\
+    (!X L E.   var X <> restr L E :'a CCS) /\
+    (!X E rf.  var X <> relab E rf :'a CCS) /\
+    (!X Y E.   var X <> rec Y E :'a CCS) /\
+    (!u E E1 E2. prefix u E <> E1 + E2 :'a CCS) /\
+    (!u E E1 E2. prefix u E <> E1 || E2 :'a CCS) /\
+    (!u E L E'.  prefix u E <> restr L E' :'a CCS) /\
+    (!u E E' rf. prefix u E <> relab E' rf :'a CCS) /\
+    (!u E X E'.  prefix u E <> rec X E' :'a CCS) /\
+    (!E1 E2 E3 E4. E1 + E2 <> E3 || E4 :'a CCS) /\
+    (!E1 E2 L E.   E1 + E2 <> restr L E :'a CCS) /\
+    (!E1 E2 E rf.  E1 + E2 <> relab E rf :'a CCS) /\
+    (!E1 E2 X E.   E1 + E2 <> rec X E :'a CCS) /\
+    (!E1 E2 L E.   E1 || E2 <> (restr L) E :'a CCS) /\
+    (!E1 E2 E rf.  E1 || E2 <> relab E rf :'a CCS) /\
+    (!E1 E2 X E.   E1 || E2 <> rec X E :'a CCS) /\
+    (!L E E' rf. restr L E <> relab E' rf :'a CCS) /\
+    (!L E X E'.  restr L E <> rec X E' :'a CCS) /\
+     !E rf X E'. relab E rf <> rec X E' :'a CCS
+Proof
+    srw_tac [] [nil_def, nil_termP, var_def, var_termP,
+                prefix_def, prefix_termP, sum_def, sum_termP,
+                par_def, par_termP, restr_def, restr_termP,
+                relab_def, relab_termP, rec_def, rec_termP,
+                term_ABS_pseudo11, gterm_distinct, GLAM_eq_thm]
+QED
 
 local
     val thm = CONJUNCTS CCS_distinct;
     val CCS_distinct_LIST = thm @ (map GSYM thm);
 in
-    val CCS_distinct' = save_thm ("CCS_distinct'", LIST_CONJ CCS_distinct_LIST);
+    val CCS_distinct' = save_thm
+      ("CCS_distinct'", LIST_CONJ CCS_distinct_LIST);
 end
 
 Theorem CCS_distinct_exists :
-    !p :('a, 'b) CCS. ?q. q <> p
+    !(p :'a CCS). ?q. q <> p
 Proof
-    GEN_TAC >> Cases_on `p` >> rpt STRIP_TAC
- >- (Q.EXISTS_TAC `prefix a nil` >> REWRITE_TAC [CCS_distinct'])
- >> Q.EXISTS_TAC `nil`
- >> REWRITE_TAC [CCS_distinct]
+    Q.X_GEN_TAC ‘p’
+ >> MP_TAC (Q.SPEC ‘p’ CCS_cases) >> rw []
+ >- (Q.EXISTS_TAC ‘prefix a nil’ >> rw [CCS_distinct'])
+ >> Q.EXISTS_TAC ‘nil’
+ >> rw [CCS_distinct]
 QED
 
-(* Prove that the constructors of the type CCS are one-to-one. *)
-val CCS_11 = TypeBase.one_one_of ``:('a, 'b) CCS``;
+Theorem CCS_distinct_exists_FV :
+    !X (p :'a CCS). ?q. q <> p /\ DISJOINT (FV q) X
+Proof
+    rw []
+ >> MP_TAC (Q.SPEC ‘p’ CCS_cases) >> rw []
+ >- (Q.EXISTS_TAC ‘prefix a nil’ >> rw [CCS_distinct'])
+ >> Q.EXISTS_TAC ‘nil’
+ >> rw [CCS_distinct]
+QED
 
-(* Given any agent expression, define the substitution of an agent expression
-   E' for an agent variable X.
+(* cf. rec_eq_thm for “rec X E = rec X' E'” *)
+Theorem CCS_one_one[simp] :
+    (!X X'. var X = var X' :'a CCS <=> X = X') /\
+    (!u E u' E' :'a CCS. prefix u E = prefix u' E' <=> u = u' /\ E = E') /\
+    (!E1 E2 E1' E2' :'a CCS. E1 + E2 = E1' + E2' <=> E1 = E1' /\ E2 = E2') /\
+    (!E1 E2 E1' E2' :'a CCS. E1 || E2 = E1' || E2' <=> E1 = E1' /\ E2 = E2') /\
+    (!L E L' E' :'a CCS. restr L E = restr L' E' <=> L = L' /\ E = E') /\
+    (!(E :'a CCS) rf E' rf'. relab E rf = relab E' rf' <=> E = E' /\ rf = rf')
+Proof
+    srw_tac [] [nil_def, nil_termP, var_def, var_termP,
+                prefix_def, prefix_termP, sum_def, sum_termP,
+                par_def, par_termP, restr_def, restr_termP,
+                relab_def, relab_termP,
+                term_ABS_pseudo11, gterm_11, term_REP_11]
+ >> rw [Once CONJ_COMM]
+QED
 
-   This works under the hypothesis that the Barendregt convention holds.
- *)
-Definition CCS_Subst_def :
+Theorem sum_acyclic :
+    !t1 t2 :'a CCS. t1 <> t1 + t2 /\ t1 <> t2 + t1
+Proof
+    HO_MATCH_MP_TAC simple_induction >> SRW_TAC [][]
+QED
+
+Theorem par_acyclic :
+    !t1 t2 :'a CCS. t1 <> t1 || t2 /\ t1 <> t2 || t1
+Proof
+    HO_MATCH_MP_TAC simple_induction >> SRW_TAC [][]
+QED
+
+Theorem FORALL_TERM :
+    (!(t :'a CCS). P t) <=>
+    P nil /\ (!s. P (var s)) /\ (!u t. P (prefix u t)) /\
+    (!t1 t2. P (t1 + t2)) /\ (!t1 t2. P (t1 || t2)) /\
+    (!L t. P (restr L t)) /\ (!t rf. P (relab t rf)) /\
+    (!v t. P (rec v t))
+Proof
+    EQ_TAC >> SRW_TAC [][]
+ >> Q.SPEC_THEN ‘t’ STRUCT_CASES_TAC CCS_cases >> SRW_TAC [][]
+QED
+
+(* ----------------------------------------------------------------------
+    Establish substitution function
+   ---------------------------------------------------------------------- *)
+
+Theorem tpm_COND[local] :
+    tpm pi (if P then x else y) = if P then tpm pi x else tpm pi y
+Proof
+    SRW_TAC [][]
+QED
+
+Theorem tpm_apart :
+    !(t :'a CCS). x NOTIN FV t /\ y IN FV t ==> tpm [(x,y)] t <> t
+Proof
+    metis_tac[supp_apart, pmact_flip_args]
+QED
+
+Theorem tpm_fresh :
+    !(t :'a CCS) x y. x NOTIN FV t /\ y NOTIN FV t ==> tpm [(x,y)] t = t
+Proof
+    srw_tac [][supp_fresh]
+QED
+
+val rewrite_pairing = prove(
+   “(?f: 'a CCS -> (string # 'a CCS) -> 'a CCS. P f) <=>
+    (?f: 'a CCS -> string -> 'a CCS -> 'a CCS. P (\M (x,N). f N x M))”,
+  EQ_TAC >> strip_tac >| [
+    qexists_tac ‘\N x M. f M (x,N)’ >> srw_tac [][] \\
+    CONV_TAC (DEPTH_CONV pairLib.PAIRED_ETA_CONV) \\
+    srw_tac [ETA_ss][],
+    qexists_tac ‘\M (x,N). f N x M’ >> srw_tac [][]
+  ]);
+
+val subst_exists =
+    parameter_tm_recursion
+        |> INST_TYPE [“:'r” |-> “:'a CCS”,
+                      “:'q” |-> “:string # 'a CCS”]
+        |> SPEC_ALL
+        |> Q.INST [‘A’ |-> ‘{}’, ‘apm’ |-> ‘^t_pmact_t’,
+                   ‘ppm’ |-> ‘pair_pmact string_pmact ^t_pmact_t’,
+                   ‘vr’ |-> ‘\s (x,N). if s = x then N else var s’,
+                   ‘nl’ |-> ‘\r. nil’,
+                   ‘pf’ |-> ‘\r x t p. prefix x (r p)’,
+                   ‘sm’ |-> ‘\r1 r2 t1 t2 p. r1 p + r2 p’,
+                   ‘pr’ |-> ‘\r1 r2 t1 t2 p. r1 p || r2 p’,
+                   ‘rs’ |-> ‘\r L t p. restr L (r p)’,
+                   ‘rl’ |-> ‘\r t rf p. relab (r p) rf’,
+                   ‘re’ |-> ‘\r s t p. rec s (r p)’]
+        |> CONV_RULE (LAND_CONV (SIMP_CONV (srw_ss()) [pairTheory.FORALL_PROD]))
+        |> SIMP_RULE (srw_ss()) [support_def, FUN_EQ_THM, fnpm_def,
+                                 tpm_COND, tpm_fresh, pmact_sing_inv,
+                                 basic_swapTheory.swapstr_eq_left]
+        |> SIMP_RULE (srw_ss()) [rewrite_pairing, pairTheory.FORALL_PROD]
+        |> CONV_RULE (DEPTH_CONV (rename_vars [("p_1", "u"), ("p_2", "E")]))
+        |> prove_alpha_fcbhyp {ppm = ``pair_pmact string_pmact ^t_pmact_t``,
+                               rwts = [],
+                               alphas = [tpm_ALPHA]};
+
+val SUB_DEF = new_specification("SUB_DEF", ["SUB"], subst_exists);
+
+val _ = add_rule {term_name = "SUB", fixity = Closefix,
+                  pp_elements = [TOK "[", TM, TOK "/", TM, TOK "]"],
+                  paren_style = OnlyIfNecessary,
+                  block_style = (AroundEachPhrase, (PP.INCONSISTENT, 2))};
+
+val _ = TeX_notation { hol = "[", TeX = ("\\ensuremath{[}", 1) };
+val _ = TeX_notation { hol = "/", TeX = ("\\ensuremath{/}", 1) };
+val _ = TeX_notation { hol = "]", TeX = ("\\ensuremath{]}", 1) };
+
+val SUB_THMv = prove(
+  “([N/x](var x) = (N :'a CCS)) /\ (x <> y ==> [N/y](var x) = var x)”,
+  SRW_TAC [][SUB_DEF]);
+
+val SUB_COMM = prove(
+   “!N x x' y (t :'a CCS).
+        x' <> x /\ x' # N ∧ y <> x /\ y # N ==>
+        (tpm [(x',y)] ([N/x] t) = [N/x] (tpm [(x',y)] t))”,
+  srw_tac [][SUB_DEF, supp_fresh]);
+
+val SUB_THM = save_thm("SUB_THM",
+  let val (eqns,_) = CONJ_PAIR SUB_DEF
+  in
+    CONJ (REWRITE_RULE [GSYM CONJ_ASSOC]
+                       (LIST_CONJ (SUB_THMv :: tl (CONJUNCTS eqns))))
+         SUB_COMM
+  end);
+val _ = export_rewrites ["SUB_THM"];
+
+(* |- !Y X E. [E/X] (var Y) = if Y = X then E else var Y *)
+Theorem SUB_VAR = hd (CONJUNCTS SUB_DEF) |> Q.SPECL [‘Y’, ‘X’] |> GEN_ALL
+
+(* |- !Y X E' E. Y <> X /\ Y # E' ==> [E'/X] (rec Y E) = rec Y ([E'/X] E) *)
+Theorem SUB_REC = List.nth (CONJUNCTS SUB_DEF, 7)
+               |> Q.SPECL [‘Y’, ‘X’, ‘E'’, ‘E’] |> GEN_ALL
+
+(* ----------------------------------------------------------------------
+    Results about substitution
+   ---------------------------------------------------------------------- *)
+
+Theorem fresh_tpm_subst :
+    !t. u # (t :'a CCS) ==> (tpm [(u,v)] t = [var u/v] t)
+Proof
+    HO_MATCH_MP_TAC CCS_induction >> Q.EXISTS_TAC ‘{u;v}’
+ >> SRW_TAC [][SUB_THM, SUB_VAR]
+QED
+
+Theorem tpm_subst :
+    !N :'a CCS. tpm pi ([M/v] N) = [tpm pi M/lswapstr pi v] (tpm pi N)
+Proof
+    HO_MATCH_MP_TAC CCS_induction
+ >> Q.EXISTS_TAC ‘v INSERT FV M’
+ >> SRW_TAC [][SUB_THM, SUB_VAR]
+QED
+
+Theorem tpm_subst_out :
+    [M/v] (tpm pi (N :'a CCS)) =
+    tpm pi ([tpm (REVERSE pi) M/lswapstr (REVERSE pi) v] N)
+Proof
+    SRW_TAC [][tpm_subst]
+QED
+
+Theorem lemma14a[simp] :
+    !t. [var v/v] t = (t :'a CCS)
+Proof
+    HO_MATCH_MP_TAC CCS_induction >> Q.EXISTS_TAC ‘{v}’
+ >> SRW_TAC [][SUB_THM, SUB_VAR]
+QED
+
+Theorem lemma14b :
+    !M. v # M ==> [N/v] M = (M :'a CCS)
+Proof
+    HO_MATCH_MP_TAC CCS_induction >> Q.EXISTS_TAC ‘v INSERT FV N’
+ >> SRW_TAC [][SUB_THM, SUB_VAR]
+QED
+
+Theorem lemma14c :
+    !t x u :'a CCS. x IN FV u ==> (FV ([t/x]u) = FV t UNION (FV u DELETE x))
+Proof
+    NTAC 2 GEN_TAC
+ >> HO_MATCH_MP_TAC CCS_induction
+ >> Q.EXISTS_TAC ‘x INSERT FV t’
+ >> SRW_TAC [][SUB_THM, SUB_VAR, EXTENSION]
+ >> METIS_TAC [lemma14b]
+QED
+
+Theorem FV_SUB :
+    !(t :'a CCS) u v. FV ([t/v] u) =
+                      if v IN FV u then FV t UNION (FV u DELETE v) else FV u
+Proof
+    PROVE_TAC [lemma14b, lemma14c]
+QED
+
+Theorem lemma15a :
+    !M :'a CCS. v # M ==> [N/v] ([var v/x] M) = [N/x] M
+Proof
+    HO_MATCH_MP_TAC CCS_induction >> Q.EXISTS_TAC ‘{x;v} UNION FV N’
+ >> SRW_TAC [][SUB_THM, SUB_VAR]
+QED
+
+Theorem lemma15b :
+    v # (M :'a CCS) ==> [var u/v] ([var v/u] M) = M
+Proof
+    SRW_TAC [][lemma15a]
+QED
+
+Theorem SUB_TWICE_ONE_VAR :
+    !M :'a CCS. [x/v] ([y/v] M) = [[x/v] y/v] M
+Proof
+    HO_MATCH_MP_TAC CCS_induction
+ >> SRW_TAC [][SUB_THM, SUB_VAR]
+ >> Q.EXISTS_TAC ‘v INSERT FV x UNION FV y’
+ >> SRW_TAC [][SUB_THM]
+ >> Cases_on ‘v IN FV y’
+ >> SRW_TAC [][SUB_THM, lemma14c, lemma14b]
+QED
+
+Theorem swap_eq_3substs :
+    z # (M :'a CCS) /\ x <> z /\ y <> z ==>
+    tpm [(x,y)] M = [var y/z] ([var x/y] ([var z/x] M))
+Proof
+    SRW_TAC [][GSYM fresh_tpm_subst]
+ >> ‘tpm [(x,y)] (tpm [(z,x)] M) =
+     tpm [(swapstr x y z, swapstr x y x)] (tpm [(x,y)] M)’
+     by (SRW_TAC [][Once (GSYM pmact_sing_to_back), SimpLHS] \\
+         SRW_TAC [][])
+ >> POP_ASSUM SUBST_ALL_TAC
+ >> SRW_TAC [][pmact_flip_args]
+QED
+
+(* ----------------------------------------------------------------------
+    alpha-convertibility results
+   ---------------------------------------------------------------------- *)
+
+Theorem SIMPLE_ALPHA :
+    y # (u :'a CCS) ==> !x. rec x u = rec y ([var y/x] u)
+Proof
+    SRW_TAC [][GSYM fresh_tpm_subst]
+ >> SRW_TAC [boolSimps.CONJ_ss][rec_eq_thm, pmact_flip_args]
+QED
+
+(* ----------------------------------------------------------------------
+    size function
+   ---------------------------------------------------------------------- *)
+
+val size_exists =
+    tm_recursion
+        |> INST_TYPE [“:'r” |-> “:num”]
+        |> SPEC_ALL
+        |> Q.INST [‘A’ |-> ‘{}’, ‘apm’ |-> ‘discrete_pmact’,
+                   ‘vr’ |-> ‘\s. 1’,
+                   ‘nl’ |-> ‘1’,
+                   ‘pf’ |-> ‘\m u E. m + 1’,
+                   ‘sm’ |-> ‘\m n t1 t2. m + n + 1’,
+                   ‘pr’ |-> ‘\m n t1 t2. m + n + 1’,
+                   ‘rs’ |-> ‘\m L t. m + 1’,
+                   ‘rl’ |-> ‘\m t rf. m + 1’,
+                   ‘re’ |-> ‘\m v t. m + 1’]
+        |> SIMP_RULE (srw_ss()) []
+
+val size_def = new_specification("CCS_size_def", ["CCS_size"], size_exists);
+
+Theorem size_thm[simp] = CONJUNCT1 size_def
+
+Theorem size_tpm[simp] = GSYM (CONJUNCT2 size_def)
+
+Theorem size_nonzero :
+    !t :'a CCS. 0 < CCS_size t
+Proof
+    HO_MATCH_MP_TAC simple_induction
+ >> SRW_TAC [ARITH_ss][]
+QED
+
+(* |- !t. CCS_size t <> 0 *)
+Theorem size_nz =
+    REWRITE_RULE [GSYM arithmeticTheory.NOT_ZERO_LT_ZERO] size_nonzero
+
+Theorem size_vsubst[simp]:
+    !M :'a CCS. CCS_size ([var v/u] M) = CCS_size M
+Proof
+    HO_MATCH_MP_TAC CCS_induction >> Q.EXISTS_TAC ‘{u;v}’
+ >> SRW_TAC [][SUB_VAR, SUB_THM]
+QED
+
+(* ----------------------------------------------------------------------
+    CCS_Subst (obsoleted)
+   ---------------------------------------------------------------------- *)
+
+Definition CCS_Subst :
+    CCS_Subst E E' X = [E'/X] (E :'a CCS)
+End
+
+(* NOTE: “Y # E'” is additionally required in case of ‘rec’ *)
+Theorem CCS_Subst_def :
    (CCS_Subst nil          E' X = nil) /\
    (CCS_Subst (prefix u E) E' X = prefix u (CCS_Subst E E' X)) /\
    (CCS_Subst (sum E1 E2)  E' X = sum (CCS_Subst E1 E' X)
@@ -121,9 +919,11 @@ Definition CCS_Subst_def :
    (CCS_Subst (restr L E)  E' X = restr L (CCS_Subst E E' X)) /\
    (CCS_Subst (relab E rf) E' X = relab   (CCS_Subst E E' X) rf) /\
    (CCS_Subst (var Y)      E' X = if (Y = X) then E' else (var Y)) /\
-   (CCS_Subst (rec Y E)    E' X = if (Y = X) then (rec Y E)
-                                  else (rec Y (CCS_Subst E E' X)))
-End
+   (Y <> X /\ Y # E' ==>
+    CCS_Subst (rec Y E)    E' X = rec Y (CCS_Subst E E' X))
+Proof
+    rw [CCS_Subst]
+QED
 
 val [CCS_Subst_nil,   CCS_Subst_prefix, CCS_Subst_sum, CCS_Subst_par,
      CCS_Subst_restr, CCS_Subst_relab,  CCS_Subst_var, CCS_Subst_rec] =
@@ -134,497 +934,64 @@ val [CCS_Subst_nil,   CCS_Subst_prefix, CCS_Subst_sum, CCS_Subst_par,
                    "CCS_Subst_var",   "CCS_Subst_rec"],
                   CONJUNCTS CCS_Subst_def));
 
-(* `[E'/X] E`, learnt from <holdir>/examples/lambda/basics/termScript.sml *)
-val _ = overload_on ("SUB", ``\E' X E. CCS_Subst E E' X``);
+(* 1st fixed point of CCS_Subst *)
+Theorem CCS_Subst_rec_fix[simp] :
+    !X E E'. CCS_Subst (rec X E) E' X = rec X E
+Proof
+    rw [CCS_Subst] >> MATCH_MP_TAC lemma14b >> rw []
+QED
 
-val _ = TeX_notation { hol = "[", TeX = ("\\ensuremath{[}", 1) };
-val _ = TeX_notation { hol = "/", TeX = ("\\ensuremath{/}", 1) };
-val _ = TeX_notation { hol = "]", TeX = ("\\ensuremath{]}", 1) };
+(* 2nd fixed point of CCS_Subst *)
+Theorem CCS_Subst_var_fix[simp] :
+    !X E. CCS_Subst (var X) E X = E
+Proof
+    rw [CCS_Subst_var]
+QED
 
-(* Note that in the rec clause, if Y = X then all occurrences of Y in E are X
-   and bound, so there exist no free variables X in E to be replaced with E'.
-   Hence, the term rec Y E is returned.
-
-   Below are two typical cases by CCS_Subst: *)
-
-(* !X E E'. CCS_Subst (rec X E) E' X = rec X E (1st fixed point of CCS_Subst) *)
-val CCS_Subst_rec_fix = save_thm (
-   "CCS_Subst_rec_fix[simp]",
-    Q.GENL [`X`, `E`, `E'`]
-           (REWRITE_CONV [CCS_Subst_def] ``CCS_Subst (rec X E) E' X``));
-
-(* !X E. CCS_Subst (var X) E X = E             (2nd fixed point of CCS_Subst) *)
-val CCS_Subst_var_fix = save_thm (
-   "CCS_Subst_var_fix[simp]",
-    Q.GENL [`X`, `E`]
-           (REWRITE_CONV [CCS_Subst_def] ``CCS_Subst (var X) E X``));
-
-Theorem CCS_Subst_self[simp] :                    (* (3rd fixed point of CCS_Subst) *)
+(* 3rd fixed point of CCS_Subst *)
+Theorem CCS_Subst_self[simp] :
     !X E. CCS_Subst E (var X) X = E
 Proof
-    GEN_TAC >> Induct_on `E` >> RW_TAC std_ss [CCS_Subst_def]
+    rw [CCS_Subst]
 QED
 
-(* !t1 t2. ((T => t1 | t2) = t1) /\ ((F => t1 | t2) = t2) *)
-val CCS_COND_CLAUSES = save_thm (
-   "CCS_COND_CLAUSES", INST_TYPE [``:'a`` |-> ``:('a, 'b) CCS``] COND_CLAUSES);
+(* !t1 t2. (if T then t1 else t2) = t1) /\ (if F then t1 else t2) = t2) *)
+Theorem CCS_COND_CLAUSES = INST_TYPE [“:'a” |-> “:'a CCS”] COND_CLAUSES
 
-(******************************************************************************)
-(*                                                                            *)
-(*            Definition of the transition relation for pure CCS              *)
-(*                                                                            *)
-(******************************************************************************)
+(* ----------------------------------------------------------------------
+    Set up the recursion functionality in binderLib
+   ---------------------------------------------------------------------- *)
 
-val _ = type_abbrev_pp ("transition",
-      ``:('a, 'b) CCS -> 'b Action -> ('a, 'b) CCS -> bool``);
+val lemma = prove(
+   “(!x y t. pmact apm [(x,y)] (h t) = h (tpm [(x,y)] t)) <=>
+     !pi t. pmact apm pi (h t) = h (tpm pi t)”,
+    simp_tac (srw_ss()) [EQ_IMP_THM]
+ >> ONCE_REWRITE_TAC [EQ_SYM_EQ]
+ >> strip_tac >> Induct_on ‘pi’
+ >> asm_simp_tac (srw_ss()) [pmact_nil, pairTheory.FORALL_PROD]
+ >> srw_tac [][Once tpm_CONS] >> srw_tac [][GSYM pmact_decompose]);
 
-(* Inductive definition of the transition relation TRANS for CCS.
-   TRANS: CCS -> Action -> CCS -> bool
- *)
-Inductive TRANS :
-    (!E u.                           TRANS (prefix u E) u E) /\         (* PREFIX *)
-    (!E u E1 E'.    TRANS E u E1 ==> TRANS (sum E E') u E1) /\          (* SUM1 *)
-    (!E u E1 E'.    TRANS E u E1 ==> TRANS (sum E' E) u E1) /\          (* SUM2 *)
-    (!E u E1 E'.    TRANS E u E1 ==> TRANS (par E E') u (par E1 E')) /\ (* PAR1 *)
-    (!E u E1 E'.    TRANS E u E1 ==> TRANS (par E' E) u (par E' E1)) /\ (* PAR2 *)
-    (!E l E1 E' E2. TRANS E (label l) E1 /\ TRANS E' (label (COMPL l)) E2
-                ==> TRANS (par E E') tau (par E1 E2)) /\                (* PAR3 *)
-    (!E u E' l L.   TRANS E u E' /\ ((u = tau) \/
-                                     ((u = label l) /\ l NOTIN L /\ (COMPL l) NOTIN L))
-                ==> TRANS (restr L E) u (restr L E')) /\                (* RESTR *)
-    (!E u E' rf.    TRANS E u E'
-                ==> TRANS (relab E rf) (relabel rf u) (relab E' rf)) /\ (* RELABELING *)
-    (!E u X E1.     TRANS (CCS_Subst E (rec X E) X) u E1
-                ==> TRANS (rec X E) u E1)                               (* REC *)
-End
+Theorem tm_recursion_nosideset =
+  tm_recursion |> Q.INST [‘A’ |-> ‘{}’] |> SIMP_RULE (srw_ss()) [lemma]
 
-val _ =
-    add_rule { term_name = "TRANS", fixity = Infix (NONASSOC, 450),
-        pp_elements = [ BreakSpace(1,0), TOK "--", HardSpace 0, TM, HardSpace 0,
-                        TOK "->", BreakSpace(1,0) ],
-        paren_style = OnlyIfNecessary,
-        block_style = (AroundEachPhrase, (PP.CONSISTENT, 0)) };
+val term_info_string =
+    "local\n\
+    \fun k |-> v = {redex = k, residue = v}\n\
+    \open binderLib\n\
+    \val term_info = \n\
+    \   {nullfv = “rec \"\" (var \"\") :'a CCS”,\n\
+    \    pm_rewrites = [],\n\
+    \    pm_constant = “(nomset$mk_pmact CCS$raw_tpm) :'a CCS pmact”,\n\
+    \    fv_rewrites = [],\n\
+    \    recursion_thm = SOME tm_recursion_nosideset,\n\
+    \    binders = [(“CCS$rec :string -> 'a CCS -> 'a CCS”, 0, tpm_ALPHA)]}\n\
+    \val _ = binderLib.type_db :=\n\
+    \          Binarymap.insert(!binderLib.type_db,\n\
+    \                           {Thy=\"CCS\", Name = \"CCS\"},\n\
+    \                           binderLib.NTI term_info)\n\
+    \in end;\n";
 
-val _ = TeX_notation { hol = "--", TeX = ("\\HOLTokenTransBegin", 1) };
-val _ = TeX_notation { hol = "->", TeX = ("\\HOLTokenTransEnd", 1) };
-
-(* The rules for the transition relation TRANS as individual theorems. *)
-val [PREFIX, SUM1, SUM2, PAR1, PAR2, PAR3, RESTR, RELABELING, REC] =
-    map save_thm
-        (combine (["PREFIX", "SUM1", "SUM2", "PAR1", "PAR2", "PAR3", "RESTR",
-                   "RELABELING", "REC"],
-                  CONJUNCTS TRANS_rules));
-
-val TRANS_IND = save_thm ("TRANS_IND",
-    TRANS_ind |> (Q.SPEC `P`) |> GEN_ALL);
-
-(* The process nil has no transitions.
-   !u E. ~TRANS nil u E
- *)
-val NIL_NO_TRANS = save_thm ("NIL_NO_TRANS",
-    Q.GENL [`u`, `E`]
-           (REWRITE_RULE [CCS_distinct]
-                         (SPECL [``nil``, ``u :'b Action``, ``E :('a, 'b) CCS``] TRANS_cases)));
-
-(* !u E. nil --u-> E <=> F *)
-val NIL_NO_TRANS_EQF = save_thm (
-   "NIL_NO_TRANS_EQF",
-    Q.GENL [`u`, `E`] (EQF_INTRO (SPEC_ALL NIL_NO_TRANS)));
-
-(* If a process can do an action, the process is not `nil`. *)
-Theorem TRANS_IMP_NO_NIL :
-    !E u E'. TRANS E u E' ==> E <> nil
-Proof
-    PROVE_TAC [NIL_NO_TRANS]
-QED
-
-(* An recursion variable has no transition.
-   !X u E. ~TRANS (var X) u E
- *)
-val VAR_NO_TRANS = save_thm ("VAR_NO_TRANS",
-    Q.GENL [`X`, `u`, `E`]
-           (REWRITE_RULE [CCS_distinct', CCS_11]
-                         (Q.SPECL [`var X`, `u`, `E`] TRANS_cases)));
-
-(* !u E u' E'. TRANS (prefix u E) u' E' = (u' = u) /\ (E' = E) *)
-val TRANS_PREFIX_EQ = save_thm (
-   "TRANS_PREFIX_EQ",
-  ((Q.GENL [`u`, `E`, `u'`, `E'`]) o
-   (ONCE_REWRITE_RHS_RULE [EQ_SYM_EQ]) o
-   SPEC_ALL o
-   (REWRITE_RULE [CCS_distinct', CCS_11]))
-      (SPECL [``prefix (u :'b Action) E``, ``u' :'b Action``, ``E' :('a, 'b) CCS``]
-             TRANS_cases));
-
-(* !u E u' E'. u..E --u'-> E' ==> (u' = u) /\ (E' = E) *)
-val TRANS_PREFIX = save_thm (
-   "TRANS_PREFIX", EQ_IMP_LR TRANS_PREFIX_EQ);
-
-(******************************************************************************)
-(*                                                                            *)
-(*                The transitions of a binary summation                       *)
-(*                                                                            *)
-(******************************************************************************)
-
-(* !P P' u P''.
-         P + P' --u-> P'' <=>
-         (?E E'. (P = E /\ P' = E') /\ E --u-> P'') \/
-          ?E E'. (P = E' /\ P' = E) /\ E --u-> P''
- *)
-val SUM_cases_EQ = save_thm (
-   "SUM_cases_EQ",
-    Q.GENL [`P`, `P'`, `u`, `P''`]
-         (REWRITE_RULE [CCS_distinct', CCS_11]
-                       (SPECL [``sum P P'``, ``u :'b Action``, ``P'' :('a, 'b) CCS``]
-                              TRANS_cases)));
-
-val SUM_cases = save_thm (
-   "SUM_cases", EQ_IMP_LR SUM_cases_EQ);
-
-Theorem TRANS_SUM_EQ :
-    !E E' u E''. TRANS (sum E E') u E'' <=> TRANS E u E'' \/ TRANS E' u E''
-Proof
-    rpt GEN_TAC
- >> EQ_TAC (* 2 sub-goals here *)
- >| [ (* goal 1 (of 2) *)
-      DISCH_TAC \\
-      IMP_RES_TAC SUM_cases >> art [],
-      (* goal 2 (of 2) *)
-      STRIP_TAC >| (* 2 sub-goals here *)
-      [ MATCH_MP_TAC SUM1 >> art [],
-        MATCH_MP_TAC SUM2 >> art [] ] ]
-QED
-
-(* for CCS_TRANS_CONV *)
-val TRANS_SUM_EQ' = store_thm (
-   "TRANS_SUM_EQ'",
-  ``!E1 E2 u E. TRANS (sum E1 E2) u E <=> TRANS E1 u E \/ TRANS E2 u E``,
-    REWRITE_TAC [TRANS_SUM_EQ]);
-
-val TRANS_SUM = save_thm (
-   "TRANS_SUM", EQ_IMP_LR TRANS_SUM_EQ);
-
-val TRANS_COMM_EQ = store_thm ("TRANS_COMM_EQ",
-  ``!E E' E'' u. TRANS (sum E E') u E'' <=> TRANS (sum E' E) u E''``,
-    rpt GEN_TAC
- >> EQ_TAC (* 2 sub-goals here *)
- >| [ (* goal 1 (of 2) *)
-      DISCH_TAC \\
-      IMP_RES_TAC TRANS_SUM >|
-      [ MATCH_MP_TAC SUM2, MATCH_MP_TAC SUM1 ] \\
-      art [],
-      (* goal 2 (of 2) *)
-      DISCH_TAC \\
-      IMP_RES_TAC TRANS_SUM >|
-      [ MATCH_MP_TAC SUM2, MATCH_MP_TAC SUM1 ] \\
-      art [] ]);
-
-val TRANS_ASSOC_EQ = store_thm ("TRANS_ASSOC_EQ",
-  ``!E E' E'' E1 u. TRANS (sum (sum E E') E'') u E1 <=> TRANS (sum E (sum E' E'')) u E1``,
-    rpt GEN_TAC
- >> EQ_TAC
- >| [ (* goal 1 (of 2) *)
-      DISCH_TAC \\
-      IMP_RES_TAC TRANS_SUM >|
-      [ (* goal 1.1 (of 2) *)
-        IMP_RES_TAC TRANS_SUM >| (* 4 sub-goals here *)
-        [ MATCH_MP_TAC SUM1,
-          MATCH_MP_TAC SUM1,
-          MATCH_MP_TAC SUM2 >> MATCH_MP_TAC SUM1,
-          MATCH_MP_TAC SUM2 >> MATCH_MP_TAC SUM1 ] \\
-        art [],
-        (* goal 1.2 (of 2) *)
-        MATCH_MP_TAC SUM2 >> MATCH_MP_TAC SUM2 \\
-        art [] ],
-      (* goal 2 (of 2) *)
-      DISCH_TAC \\
-      IMP_RES_TAC TRANS_SUM >|
-      [ MATCH_MP_TAC SUM1 >> MATCH_MP_TAC SUM1 \\
-        art [],
-        IMP_RES_TAC TRANS_SUM >| (* 4 sub-goals here *)
-        [ MATCH_MP_TAC SUM1 >> MATCH_MP_TAC SUM1,
-          MATCH_MP_TAC SUM1 >> MATCH_MP_TAC SUM2,
-          MATCH_MP_TAC SUM2,
-          MATCH_MP_TAC SUM2 ] >> art [] ] ]);
-
-val TRANS_ASSOC_RL = save_thm (
-   "TRANS_ASSOC_RL", EQ_IMP_RL TRANS_ASSOC_EQ);
-
-val TRANS_SUM_NIL_EQ = store_thm (
-   "TRANS_SUM_NIL_EQ",
-  ``!E u E'. TRANS (sum E nil) u E' <=> TRANS E u E'``,
-    rpt GEN_TAC
- >> EQ_TAC (* 2 sub-goals here *)
- >| [ (* goal 1 (of 2) *)
-      DISCH_TAC \\
-      IMP_RES_TAC TRANS_SUM \\
-      IMP_RES_TAC NIL_NO_TRANS,
-      (* goal 2 (of 2) *)
-      DISCH_TAC \\
-      MATCH_MP_TAC SUM1 >> art [] ]);
-
-(* !E u E'. E + nil --u-> E' ==> E --u-> E' *)
-val TRANS_SUM_NIL = save_thm ("TRANS_SUM_NIL", EQ_IMP_LR TRANS_SUM_NIL_EQ);
-
-val TRANS_P_SUM_P_EQ = store_thm ("TRANS_P_SUM_P_EQ",
-  ``!E u E'. TRANS (sum E E) u E' = TRANS E u E'``,
-    rpt GEN_TAC
- >> EQ_TAC
- >| [ DISCH_TAC \\
-      IMP_RES_TAC TRANS_SUM,
-      DISCH_TAC \\
-      MATCH_MP_TAC SUM1 >> art [] ]);
-
-val TRANS_P_SUM_P = save_thm
-  ("TRANS_P_SUM_P", EQ_IMP_LR TRANS_P_SUM_P_EQ);
-
-val PAR_cases_EQ = save_thm ("PAR_cases_EQ",
-    Q.GENL [`P`, `P'`, `u`, `P''`]
-        (REWRITE_RULE [CCS_distinct', CCS_11]
-                      (Q.SPECL [`par P P'`, `u`, `P''`] TRANS_cases)));
-
-val PAR_cases = save_thm ("PAR_cases", EQ_IMP_LR PAR_cases_EQ);
-
-(* NOTE: the shape of this theorem can be easily derived from above definition
-   by replacing REWRITE_RULE with SIMP_RULE, however the inner existential
-   variable (E1) has a different name. *)
-Theorem TRANS_PAR_EQ :
-    !E E' u E''. TRANS (par E E') u E'' <=>
-                 (?E1. (E'' = par E1 E') /\ TRANS E u E1) \/
-                 (?E1. (E'' = par E E1) /\ TRANS E' u E1) \/
-                 (?E1 E2 l. (u = tau) /\ (E'' = par E1 E2) /\
-                            TRANS E (label l) E1 /\ TRANS E' (label (COMPL l)) E2)
-Proof
-    rpt GEN_TAC >> EQ_TAC (* 2 sub-goals here *)
- >| [ (* case 1 (LR) *)
-      STRIP_TAC \\
-      IMP_RES_TAC PAR_cases >| (* 3 sub-goals here *)
-      [ (* goal 1.1 *)
-        DISJ1_TAC \\
-        Q.EXISTS_TAC `E1` >> art [],
-        (* goal 1.2 *)
-        DISJ2_TAC >> DISJ1_TAC \\
-        Q.EXISTS_TAC `E1` >> art [],
-        (* goal 1.3 *)
-        DISJ2_TAC >> DISJ2_TAC \\
-        take [`E1`, `E2`, `l`] >> art [] ],
-      (* case 2 (RL) *)
-      STRIP_TAC >> art [] (* 3 sub-goals, same initial tactics *)
-   >| [ MATCH_MP_TAC PAR1 >> art [],
-        MATCH_MP_TAC PAR2 >> art [],
-        MATCH_MP_TAC PAR3 \\
-        Q.EXISTS_TAC `l` >> art [] ] ]
-QED
-
-val TRANS_PAR = save_thm ("TRANS_PAR", EQ_IMP_LR TRANS_PAR_EQ);
-
-val TRANS_PAR_P_NIL = store_thm ("TRANS_PAR_P_NIL",
-  ``!E u E'. TRANS (par E nil) u E' ==> (?E''. TRANS E u E'' /\ (E' = par E'' nil))``,
-    rpt STRIP_TAC
- >> IMP_RES_TAC TRANS_PAR
- >| [ Q.EXISTS_TAC `E1` >> art [],
-      IMP_RES_TAC NIL_NO_TRANS,
-      IMP_RES_TAC NIL_NO_TRANS ]);
-
-val TRANS_PAR_NO_SYNCR = store_thm ("TRANS_PAR_NO_SYNCR",
-  ``!(l :'b Label) l'. l <> COMPL l' ==>
-        !E E' E''. ~(TRANS (par (prefix (label l) E) (prefix (label l') E')) tau E'')``,
-    rpt STRIP_TAC
- >> IMP_RES_TAC TRANS_PAR (* 3 sub-goals here *)
- >| [ IMP_RES_TAC TRANS_PREFIX >> IMP_RES_TAC Action_distinct,
-      IMP_RES_TAC TRANS_PREFIX >> IMP_RES_TAC Action_distinct,
-      IMP_RES_TAC TRANS_PREFIX >> IMP_RES_TAC Action_11 \\
-      CHECK_ASSUME_TAC
-        (REWRITE_RULE [SYM (ASSUME ``(l'' :'b Label) = l``),
-                       SYM (ASSUME ``COMPL (l'' :'b Label) = l'``), COMPL_COMPL_LAB]
-                      (ASSUME ``~(l = COMPL (l' :'b Label))``)) \\
-      RW_TAC bool_ss [] ]);
-
-val RESTR_cases_EQ = save_thm (
-   "RESTR_cases_EQ",
-    Q.GENL [`P'`, `u`, `L`, `P`]
-           (REWRITE_RULE [CCS_distinct', CCS_11, Action_distinct, Action_11]
-                         (Q.SPECL [`restr L P`, `u`, `P'`] TRANS_cases)));
-
-val RESTR_cases = save_thm (
-   "RESTR_cases", EQ_IMP_LR RESTR_cases_EQ);
-
-Theorem TRANS_RESTR_EQ :
-    !E L u E'.
-     TRANS (restr L E) u E' <=>
-     ?E'' l. (E' = restr L E'') /\ TRANS E u E'' /\
-             ((u = tau) \/ ((u = label l) /\ l NOTIN L /\ (COMPL l) NOTIN L))
-Proof
-  let val a1 = ASSUME ``(u :'b Action) = tau``
-      and a2 = ASSUME ``u = label (l :'b Label)``
-      and a3 = ASSUME ``TRANS E'' u E'''``
-      and a4 = ASSUME ``TRANS E u E''``
-  in
-    rpt GEN_TAC
- >> EQ_TAC >| (* two goals here *)
-    [ (* case 1 (LR) *)
-      STRIP_TAC \\
-      IMP_RES_TAC RESTR_cases \\ (* two sub-goals here, first two steps are shared *)
-      take [`E'''`, `l`] >|
-      [ (* goal 1.1 *)
-        art [REWRITE_RULE [a1] a3],
-        (* goal 1.2 *)
-        art [REWRITE_RULE [a2] a3] ],
-      (* case 2 (RL) *)
-      STRIP_TAC >> art [] >| (* two sub-goals here *)
-      [ (* sub-goal 2.1 *)
-        MATCH_MP_TAC RESTR \\
-        art [REWRITE_RULE [a1] a4],
-        (* sub-goal 2.2 *)
-        MATCH_MP_TAC RESTR \\
-        Q.EXISTS_TAC `l` \\
-        art [REWRITE_RULE [a2] a4] ] ]
-  end
-QED
-
-val TRANS_RESTR = save_thm (
-   "TRANS_RESTR", EQ_IMP_LR TRANS_RESTR_EQ);
-
-val TRANS_P_RESTR = store_thm (
-   "TRANS_P_RESTR",
-  ``!E u E' L. TRANS (restr L E) u (restr L E') ==> TRANS E u E'``,
-  let
-      val thm = REWRITE_RULE [CCS_11] (ASSUME ``restr (L :'b Label set) E' = restr L E''``)
-  in
-      rpt STRIP_TAC \\
-      IMP_RES_TAC TRANS_RESTR >| (* 2 sub-goals here *)
-      [ FILTER_ASM_REWRITE_TAC (fn t => t !~ ``(u :'b Action) = tau``) [thm],
-        FILTER_ASM_REWRITE_TAC (fn t => t !~ ``(u :'b Action) = label l``) [thm]
-      ]
-  end);
-
-val RESTR_NIL_NO_TRANS = store_thm ("RESTR_NIL_NO_TRANS",
-  ``!(L :'b Label set) u E. ~(TRANS (restr L nil) u E)``,
-    rpt STRIP_TAC
- >> IMP_RES_TAC TRANS_RESTR (* two sub-goals here, but same proofs *)
- >> IMP_RES_TAC NIL_NO_TRANS);
-
-val TRANS_IMP_NO_RESTR_NIL = store_thm ("TRANS_IMP_NO_RESTR_NIL",
-  ``!E u E'. TRANS E u E' ==> !L. ~(E = restr L nil)``,
-    rpt STRIP_TAC
- >> ASSUME_TAC (REWRITE_RULE [ASSUME ``E = restr L nil``]
-                             (ASSUME ``TRANS E u E'``))
- >> IMP_RES_TAC RESTR_NIL_NO_TRANS);
-
-val TRANS_RESTR_NO_NIL = store_thm ("TRANS_RESTR_NO_NIL",
-  ``!E L u E'. TRANS (restr L E) u (restr L E') ==> ~(E = nil)``,
-    rpt STRIP_TAC
- >> IMP_RES_TAC TRANS_RESTR
- >> ASSUME_TAC (REWRITE_RULE [ASSUME ``E = nil``]
-                             (ASSUME ``TRANS E u E''``))
- >> IMP_RES_TAC NIL_NO_TRANS);
-
-val RESTR_LABEL_NO_TRANS = store_thm ("RESTR_LABEL_NO_TRANS",
-  ``!(l :'b Label) L. (l IN L) \/ ((COMPL l) IN L) ==>
-                      (!E u E'. ~(TRANS (restr L (prefix (label l) E)) u E'))``,
-    rpt STRIP_TAC (* 2 goals here *)
- >| [ (* goal 1 *)
-      IMP_RES_TAC TRANS_RESTR >| (* 2 sub-goals here *)
-      [ (* goal 1.1 *)
-        IMP_RES_TAC TRANS_PREFIX \\
-        CHECK_ASSUME_TAC
-          (REWRITE_RULE [ASSUME ``(u :'b Action) = tau``, Action_distinct]
-                        (ASSUME ``(u :'b Action) = label l``)),
-        (* goal 1.2 *)
-        IMP_RES_TAC TRANS_PREFIX \\
-        CHECK_ASSUME_TAC
-          (MP (REWRITE_RULE
-                [REWRITE_RULE [ASSUME ``(u :'b Action) = label l'``, Action_11]
-                              (ASSUME ``(u :'b Action) = label l``)]
-                (ASSUME ``~((l' :'b Label) IN L)``))
-              (ASSUME ``(l :'b Label) IN L``)) ],
-      (* goal 2 *)
-      IMP_RES_TAC TRANS_RESTR >| (* 2 sub-goals here *)
-      [ (* goal 2.1 *)
-        IMP_RES_TAC TRANS_PREFIX \\
-        CHECK_ASSUME_TAC
-          (REWRITE_RULE [ASSUME ``(u :'b Action) = tau``, Action_distinct]
-                        (ASSUME ``(u :'b Action) = label l``)),
-        (* goal 2.2 *)
-        IMP_RES_TAC TRANS_PREFIX \\
-        CHECK_ASSUME_TAC
-          (MP (REWRITE_RULE
-                [REWRITE_RULE [ASSUME ``(u :'b Action) = label l'``, Action_11]
-                              (ASSUME ``(u :'b Action) = label l``)]
-                (ASSUME ``~((COMPL (l' :'b Label)) IN L)``))
-              (ASSUME ``(COMPL (l :'b Label)) IN L``)) ] ]);
-
-(* |- !E rf u P.
-         relab E rf --u-> P <=>
-         ?E' u' E'' rf'.
-             ((E = E') /\ (rf = rf')) /\ (u = relabel rf' u') /\
-             (P = relab E'' rf') /\ E' --u'-> E''
- *)
-val RELAB_cases_EQ = save_thm
-  ("RELAB_cases_EQ",
-    TRANS_cases |> (Q.SPEC `relab E rf`)
-                |> (REWRITE_RULE [CCS_distinct', CCS_11])
-                |> (Q.SPECL [`u`, `P`])
-                |> (Q.GENL [`E`, `rf`, `u`, `P`]));
-
-val RELAB_cases = save_thm ("RELAB_cases", EQ_IMP_LR RELAB_cases_EQ);
-
-Theorem TRANS_RELAB_EQ :
-    !E rf u E'. TRANS (relab E rf) u E' <=>
-                ?u' E''. (u = relabel rf u') /\
-                         (E' = relab E'' rf) /\ TRANS E u' E''
-Proof
-    rpt GEN_TAC
- >> EQ_TAC (* 2 sub-goals here *)
- >| [ (* goal 1 (of 2) *)
-      DISCH_TAC \\
-      IMP_RES_TAC RELAB_cases \\
-      take [`u'`, `E'''`] >> art [],
-      (* goal 2 (of 2) *)
-      STRIP_TAC \\
-      PURE_ONCE_ASM_REWRITE_TAC [] \\
-      MATCH_MP_TAC RELABELING \\
-      PURE_ONCE_ASM_REWRITE_TAC [] ]
-QED
-
-val TRANS_RELAB = save_thm ("TRANS_RELAB", EQ_IMP_LR TRANS_RELAB_EQ);
-
-val TRANS_RELAB_labl = save_thm ("TRANS_RELAB_labl",
-    Q.GENL [`E`, `labl`] (Q.SPECL [`E`, `RELAB labl`] TRANS_RELAB));
-
-val RELAB_NIL_NO_TRANS = store_thm ("RELAB_NIL_NO_TRANS",
-  ``!(rf :'b Relabeling) u E. ~(TRANS (relab nil rf) u E)``,
-    rpt STRIP_TAC
- >> IMP_RES_TAC TRANS_RELAB
- >> IMP_RES_TAC NIL_NO_TRANS);
-
-(* |- !X E u E'.
-         rec X E --u-> E' <=>
-         ?E'' X'. ((X = X') /\ (E = E'')) /\ [rec X' E''/X'] E'' --u-> E'
- *)
-val REC_cases_EQ = save_thm
-  ("REC_cases_EQ",
-    TRANS_cases |> (Q.SPEC `rec X E`)
-                |> (REWRITE_RULE [CCS_distinct', CCS_11])
-                |> (Q.SPECL [`u`, `E'`])
-                |> (Q.GENL [`X`, `E`, `u`, `E'`]));
-
-val REC_cases = save_thm ("REC_cases", EQ_IMP_LR REC_cases_EQ);
-
-Theorem TRANS_REC_EQ :
-    !X E u E'. TRANS (rec X E) u E' <=> TRANS (CCS_Subst E (rec X E) X) u E'
-Proof
-    rpt GEN_TAC
- >> EQ_TAC
- >| [ (* goal 1 (of 2) *)
-      PURE_ONCE_REWRITE_TAC [REC_cases_EQ] \\
-      rpt STRIP_TAC \\
-      PURE_ASM_REWRITE_TAC [],
-      (* goal 2 (of 2) *)
-      PURE_ONCE_REWRITE_TAC [REC] ]
-QED
-
-val TRANS_REC = save_thm ("TRANS_REC", EQ_IMP_LR TRANS_REC_EQ);
+val _ = adjoin_after_completion (fn _ => PP.add_string term_info_string);
 
 val _ = export_theory ();
 val _ = html_theory "CCS";
