examples/CCS/TransScript.sml
@@ -1,63 +1,509 @@
-(*
- * Copyright 1991-1995  University of Cambridge (Author: Monica Nesi)
- * Copyright 2016-2017  University of Bologna, Italy (Author: Chun Tian)
- * Copyright 2018-2019  Fondazione Bruno Kessler, Italy (Author: Chun Tian)
- * Copyright 2023-2024  The Australian National University (Author: Chun Tian)
- *)
+(* ========================================================================== *)
+(* FILE          : TransScript.sml (was part of CCSScript.sml)                *)
+(* DESCRIPTION   : A formalization of the process algebra CCS in HOL          *)
+(*                                                                            *)
+(* COPYRIGHTS    : 1991-1995 University of Cambridge (Monica Nesi)            *)
+(*                 2016-2017 University of Bologna, Italy (Chun Tian)         *)
+(*                 2018-2019 Fondazione Bruno Kessler, Italy (Chun Tian)      *)
+(*                 2023-2024 Australian National University (Chun Tian)       *)
+(******************************************************************************)
 
 open HolKernel Parse boolLib bossLib;
 
-open pred_setTheory pred_setLib relationTheory optionTheory listTheory CCSLib
-     rich_listTheory;
+open pred_setTheory pred_setLib relationTheory optionTheory listTheory
+     rich_listTheory binderLib;
 
-open LabelTheory CCSTheory;
+open CCSLib LabelTheory CCSTheory;
 
 val _ = new_theory "Trans";
 
 val set_ss = std_ss ++ PRED_SET_ss;
 
-val (CCS_size_tm, CCS_size_def) = TypeBase.size_of ``:('a, 'b) CCS``;
+(******************************************************************************)
+(*                                                                            *)
+(*            Definition of the transition relation for pure CCS              *)
+(*                                                                            *)
+(******************************************************************************)
+
+Type transition[pp] = “:'a CCS -> 'a Action -> 'a CCS -> bool”
+
+(* Inductive definition of the transition relation TRANS for CCS.
+   TRANS: CCS -> Action -> CCS -> bool
+ *)
+Inductive TRANS :
+    (!E u.                           TRANS (prefix u E) u E) /\         (* PREFIX *)
+    (!E u E1 E'.    TRANS E u E1 ==> TRANS (sum E E') u E1) /\          (* SUM1 *)
+    (!E u E1 E'.    TRANS E u E1 ==> TRANS (sum E' E) u E1) /\          (* SUM2 *)
+    (!E u E1 E'.    TRANS E u E1 ==> TRANS (par E E') u (par E1 E')) /\ (* PAR1 *)
+    (!E u E1 E'.    TRANS E u E1 ==> TRANS (par E' E) u (par E' E1)) /\ (* PAR2 *)
+    (!E l E1 E' E2. TRANS E (label l) E1 /\ TRANS E' (label (COMPL l)) E2
+                ==> TRANS (par E E') tau (par E1 E2)) /\                (* PAR3 *)
+    (!E u E' l L.   TRANS E u E' /\ ((u = tau) \/
+                                     ((u = label l) /\ l NOTIN L /\ (COMPL l) NOTIN L))
+                ==> TRANS (restr L E) u (restr L E')) /\                (* RESTR *)
+    (!E u E' rf.    TRANS E u E'
+                ==> TRANS (relab E rf) (relabel rf u) (relab E' rf)) /\ (* RELABELING *)
+    (!E u X E1.     TRANS (CCS_Subst E (rec X E) X) u E1
+                ==> TRANS (rec X E) u E1)                               (* REC *)
+End
+
+val _ =
+    add_rule { term_name = "TRANS", fixity = Infix (NONASSOC, 450),
+        pp_elements = [ BreakSpace(1,0), TOK "--", HardSpace 0, TM, HardSpace 0,
+                        TOK "->", BreakSpace(1,0) ],
+        paren_style = OnlyIfNecessary,
+        block_style = (AroundEachPhrase, (PP.CONSISTENT, 0)) };
+
+val _ = TeX_notation { hol = "--", TeX = ("\\HOLTokenTransBegin", 1) };
+val _ = TeX_notation { hol = "->", TeX = ("\\HOLTokenTransEnd", 1) };
+
+(* The rules for the transition relation TRANS as individual theorems. *)
+val [PREFIX, SUM1, SUM2, PAR1, PAR2, PAR3, RESTR, RELABELING, REC] =
+    map save_thm
+        (combine (["PREFIX", "SUM1", "SUM2", "PAR1", "PAR2", "PAR3", "RESTR",
+                   "RELABELING", "REC"],
+                  CONJUNCTS TRANS_rules));
+
+val TRANS_IND = save_thm ("TRANS_IND",
+    TRANS_ind |> (Q.SPEC `P`) |> GEN_ALL);
+
+(* The process nil has no transitions.
+   !u E. ~TRANS nil u E
+ *)
+Theorem NIL_NO_TRANS =
+    TRANS_cases |> Q.SPECL [‘nil’, ‘u’, ‘E’]
+                |> REWRITE_RULE [CCS_distinct]
+                |> Q.GENL [‘u’, ‘E’]
+
+(* !u E. nil --u-> E <=> F *)
+val NIL_NO_TRANS_EQF = save_thm (
+   "NIL_NO_TRANS_EQF",
+    Q.GENL [`u`, `E`] (EQF_INTRO (SPEC_ALL NIL_NO_TRANS)));
+
+(* If a process can do an action, the process is not `nil`. *)
+Theorem TRANS_IMP_NO_NIL :
+    !E u E'. TRANS E u E' ==> E <> nil
+Proof
+    PROVE_TAC [NIL_NO_TRANS]
+QED
+
+(* An recursion variable has no transition.
+   !X u E. ~TRANS (var X) u E
+ *)
+val VAR_NO_TRANS = save_thm ("VAR_NO_TRANS",
+    Q.GENL [`X`, `u`, `E`]
+           (REWRITE_RULE [CCS_distinct', CCS_one_one]
+                         (Q.SPECL [`var X`, `u`, `E`] TRANS_cases)));
+
+(* !u E u' E'. TRANS (prefix u E) u' E' <=> (u' = u) /\ (E' = E) *)
+Theorem TRANS_PREFIX_EQ =
+        TRANS_cases |> Q.SPECL [‘prefix u E’, ‘u'’, ‘E'’]
+                    |> REWRITE_RULE [CCS_distinct', CCS_one_one]
+                    |> ONCE_REWRITE_RHS_RULE [EQ_SYM_EQ]
+                    |> Q.GENL [‘u’, ‘E’, ‘u'’, ‘E'’]
+
+(* !u E u' E'. u..E --u'-> E' ==> (u' = u) /\ (E' = E) *)
+val TRANS_PREFIX = save_thm (
+   "TRANS_PREFIX", EQ_IMP_LR TRANS_PREFIX_EQ);
+
+(******************************************************************************)
+(*                                                                            *)
+(*                The transitions of a binary summation                       *)
+(*                                                                            *)
+(******************************************************************************)
+
+(* !P P' u P''.
+         P + P' --u-> P'' <=>
+         (?E E'. (P = E /\ P' = E') /\ E --u-> P'') \/
+          ?E E'. (P = E' /\ P' = E) /\ E --u-> P''
+ *)
+Theorem SUM_cases_EQ =
+        TRANS_cases |> Q.SPECL [‘sum P P'’, ‘u’, ‘P''’]
+                    |> REWRITE_RULE [CCS_distinct', CCS_one_one]
+                    |> Q.GENL [‘P’, ‘P'’, ‘u’, ‘P''’]
+
+val SUM_cases = save_thm (
+   "SUM_cases", EQ_IMP_LR SUM_cases_EQ);
+
+Theorem TRANS_SUM_EQ :
+    !E E' u E''. TRANS (sum E E') u E'' <=> TRANS E u E'' \/ TRANS E' u E''
+Proof
+    rpt GEN_TAC
+ >> EQ_TAC (* 2 sub-goals here *)
+ >| [ (* goal 1 (of 2) *)
+      DISCH_TAC \\
+      IMP_RES_TAC SUM_cases >> art [],
+      (* goal 2 (of 2) *)
+      STRIP_TAC >| (* 2 sub-goals here *)
+      [ MATCH_MP_TAC SUM1 >> art [],
+        MATCH_MP_TAC SUM2 >> art [] ] ]
+QED
+
+(* for CCS_TRANS_CONV *)
+val TRANS_SUM_EQ' = store_thm (
+   "TRANS_SUM_EQ'",
+  ``!E1 E2 u E. TRANS (sum E1 E2) u E <=> TRANS E1 u E \/ TRANS E2 u E``,
+    REWRITE_TAC [TRANS_SUM_EQ]);
+
+val TRANS_SUM = save_thm (
+   "TRANS_SUM", EQ_IMP_LR TRANS_SUM_EQ);
+
+val TRANS_COMM_EQ = store_thm ("TRANS_COMM_EQ",
+  ``!E E' E'' u. TRANS (sum E E') u E'' <=> TRANS (sum E' E) u E''``,
+    rpt GEN_TAC
+ >> EQ_TAC (* 2 sub-goals here *)
+ >| [ (* goal 1 (of 2) *)
+      DISCH_TAC \\
+      IMP_RES_TAC TRANS_SUM >|
+      [ MATCH_MP_TAC SUM2, MATCH_MP_TAC SUM1 ] \\
+      art [],
+      (* goal 2 (of 2) *)
+      DISCH_TAC \\
+      IMP_RES_TAC TRANS_SUM >|
+      [ MATCH_MP_TAC SUM2, MATCH_MP_TAC SUM1 ] \\
+      art [] ]);
+
+val TRANS_ASSOC_EQ = store_thm ("TRANS_ASSOC_EQ",
+  ``!E E' E'' E1 u. TRANS (sum (sum E E') E'') u E1 <=> TRANS (sum E (sum E' E'')) u E1``,
+    rpt GEN_TAC
+ >> EQ_TAC
+ >| [ (* goal 1 (of 2) *)
+      DISCH_TAC \\
+      IMP_RES_TAC TRANS_SUM >|
+      [ (* goal 1.1 (of 2) *)
+        IMP_RES_TAC TRANS_SUM >| (* 4 sub-goals here *)
+        [ MATCH_MP_TAC SUM1,
+          MATCH_MP_TAC SUM1,
+          MATCH_MP_TAC SUM2 >> MATCH_MP_TAC SUM1,
+          MATCH_MP_TAC SUM2 >> MATCH_MP_TAC SUM1 ] \\
+        art [],
+        (* goal 1.2 (of 2) *)
+        MATCH_MP_TAC SUM2 >> MATCH_MP_TAC SUM2 \\
+        art [] ],
+      (* goal 2 (of 2) *)
+      DISCH_TAC \\
+      IMP_RES_TAC TRANS_SUM >|
+      [ MATCH_MP_TAC SUM1 >> MATCH_MP_TAC SUM1 \\
+        art [],
+        IMP_RES_TAC TRANS_SUM >| (* 4 sub-goals here *)
+        [ MATCH_MP_TAC SUM1 >> MATCH_MP_TAC SUM1,
+          MATCH_MP_TAC SUM1 >> MATCH_MP_TAC SUM2,
+          MATCH_MP_TAC SUM2,
+          MATCH_MP_TAC SUM2 ] >> art [] ] ]);
+
+val TRANS_ASSOC_RL = save_thm (
+   "TRANS_ASSOC_RL", EQ_IMP_RL TRANS_ASSOC_EQ);
+
+val TRANS_SUM_NIL_EQ = store_thm (
+   "TRANS_SUM_NIL_EQ",
+  ``!E u E'. TRANS (sum E nil) u E' <=> TRANS E u E'``,
+    rpt GEN_TAC
+ >> EQ_TAC (* 2 sub-goals here *)
+ >| [ (* goal 1 (of 2) *)
+      DISCH_TAC \\
+      IMP_RES_TAC TRANS_SUM \\
+      IMP_RES_TAC NIL_NO_TRANS,
+      (* goal 2 (of 2) *)
+      DISCH_TAC \\
+      MATCH_MP_TAC SUM1 >> art [] ]);
+
+(* !E u E'. E + nil --u-> E' ==> E --u-> E' *)
+val TRANS_SUM_NIL = save_thm ("TRANS_SUM_NIL", EQ_IMP_LR TRANS_SUM_NIL_EQ);
+
+val TRANS_P_SUM_P_EQ = store_thm ("TRANS_P_SUM_P_EQ",
+  ``!E u E'. TRANS (sum E E) u E' = TRANS E u E'``,
+    rpt GEN_TAC
+ >> EQ_TAC
+ >| [ DISCH_TAC \\
+      IMP_RES_TAC TRANS_SUM,
+      DISCH_TAC \\
+      MATCH_MP_TAC SUM1 >> art [] ]);
+
+val TRANS_P_SUM_P = save_thm
+  ("TRANS_P_SUM_P", EQ_IMP_LR TRANS_P_SUM_P_EQ);
+
+val PAR_cases_EQ = save_thm ("PAR_cases_EQ",
+    Q.GENL [`P`, `P'`, `u`, `P''`]
+        (REWRITE_RULE [CCS_distinct', CCS_one_one]
+                      (Q.SPECL [`par P P'`, `u`, `P''`] TRANS_cases)));
+
+val PAR_cases = save_thm ("PAR_cases", EQ_IMP_LR PAR_cases_EQ);
+
+(* NOTE: the shape of this theorem can be easily derived from above definition
+   by replacing REWRITE_RULE with SIMP_RULE, however the inner existential
+   variable (E1) has a different name. *)
+Theorem TRANS_PAR_EQ :
+    !E E' u E''. TRANS (par E E') u E'' <=>
+                 (?E1. (E'' = par E1 E') /\ TRANS E u E1) \/
+                 (?E1. (E'' = par E E1) /\ TRANS E' u E1) \/
+                 (?E1 E2 l. (u = tau) /\ (E'' = par E1 E2) /\
+                            TRANS E (label l) E1 /\ TRANS E' (label (COMPL l)) E2)
+Proof
+    rpt GEN_TAC >> EQ_TAC (* 2 sub-goals here *)
+ >| [ (* case 1 (LR) *)
+      STRIP_TAC \\
+      IMP_RES_TAC PAR_cases >| (* 3 sub-goals here *)
+      [ (* goal 1.1 *)
+        DISJ1_TAC \\
+        Q.EXISTS_TAC `E1` >> art [],
+        (* goal 1.2 *)
+        DISJ2_TAC >> DISJ1_TAC \\
+        Q.EXISTS_TAC `E1` >> art [],
+        (* goal 1.3 *)
+        DISJ2_TAC >> DISJ2_TAC \\
+        take [`E1`, `E2`, `l`] >> art [] ],
+      (* case 2 (RL) *)
+      STRIP_TAC >> art [] (* 3 sub-goals, same initial tactics *)
+   >| [ MATCH_MP_TAC PAR1 >> art [],
+        MATCH_MP_TAC PAR2 >> art [],
+        MATCH_MP_TAC PAR3 \\
+        Q.EXISTS_TAC `l` >> art [] ] ]
+QED
+
+val TRANS_PAR = save_thm ("TRANS_PAR", EQ_IMP_LR TRANS_PAR_EQ);
+
+val TRANS_PAR_P_NIL = store_thm ("TRANS_PAR_P_NIL",
+  ``!E u E'. TRANS (par E nil) u E' ==> (?E''. TRANS E u E'' /\ (E' = par E'' nil))``,
+    rpt STRIP_TAC
+ >> IMP_RES_TAC TRANS_PAR
+ >| [ Q.EXISTS_TAC `E1` >> art [],
+      IMP_RES_TAC NIL_NO_TRANS,
+      IMP_RES_TAC NIL_NO_TRANS ]);
+
+val TRANS_PAR_NO_SYNCR = store_thm ("TRANS_PAR_NO_SYNCR",
+  ``!(l :'b Label) l'. l <> COMPL l' ==>
+        !E E' E''. ~(TRANS (par (prefix (label l) E) (prefix (label l') E')) tau E'')``,
+    rpt STRIP_TAC
+ >> IMP_RES_TAC TRANS_PAR (* 3 sub-goals here *)
+ >| [ IMP_RES_TAC TRANS_PREFIX >> IMP_RES_TAC Action_distinct,
+      IMP_RES_TAC TRANS_PREFIX >> IMP_RES_TAC Action_distinct,
+      IMP_RES_TAC TRANS_PREFIX >> IMP_RES_TAC Action_11 \\
+      CHECK_ASSUME_TAC
+        (REWRITE_RULE [SYM (ASSUME ``(l'' :'b Label) = l``),
+                       SYM (ASSUME ``COMPL (l'' :'b Label) = l'``), COMPL_COMPL_LAB]
+                      (ASSUME ``~(l = COMPL (l' :'b Label))``)) \\
+      RW_TAC bool_ss [] ]);
+
+val RESTR_cases_EQ = save_thm (
+   "RESTR_cases_EQ",
+    Q.GENL [`P'`, `u`, `L`, `P`]
+           (REWRITE_RULE [CCS_distinct', CCS_one_one, Action_distinct, Action_11]
+                         (Q.SPECL [`restr L P`, `u`, `P'`] TRANS_cases)));
+
+val RESTR_cases = save_thm (
+   "RESTR_cases", EQ_IMP_LR RESTR_cases_EQ);
+
+Theorem TRANS_RESTR_EQ :
+    !E L u E'.
+     TRANS (restr L E) u E' <=>
+     ?E'' l. (E' = restr L E'') /\ TRANS E u E'' /\
+             ((u = tau) \/ ((u = label l) /\ l NOTIN L /\ (COMPL l) NOTIN L))
+Proof
+  let val a1 = ASSUME ``(u :'a Action) = tau``
+      and a2 = ASSUME ``u = label (l :'a Label)``
+      and a3 = ASSUME ``TRANS E'' u E'''``
+      and a4 = ASSUME ``TRANS E u E''``
+  in
+    rpt GEN_TAC
+ >> EQ_TAC >| (* two goals here *)
+    [ (* case 1 (LR) *)
+      STRIP_TAC \\
+      IMP_RES_TAC RESTR_cases \\ (* two sub-goals here, first two steps are shared *)
+      take [`E'''`, `l`] >|
+      [ (* goal 1.1 *)
+        art [REWRITE_RULE [a1] a3],
+        (* goal 1.2 *)
+        art [REWRITE_RULE [a2] a3] ],
+      (* case 2 (RL) *)
+      STRIP_TAC >> art [] >| (* two sub-goals here *)
+      [ (* sub-goal 2.1 *)
+        MATCH_MP_TAC RESTR \\
+        art [REWRITE_RULE [a1] a4],
+        (* sub-goal 2.2 *)
+        MATCH_MP_TAC RESTR \\
+        Q.EXISTS_TAC `l` \\
+        art [REWRITE_RULE [a2] a4] ] ]
+  end
+QED
+
+val TRANS_RESTR = save_thm (
+   "TRANS_RESTR", EQ_IMP_LR TRANS_RESTR_EQ);
+
+val TRANS_P_RESTR = store_thm (
+   "TRANS_P_RESTR",
+  ``!E u E' L. TRANS (restr L E) u (restr L E') ==> TRANS E u E'``,
+  let
+      val thm = REWRITE_RULE [CCS_one_one]
+                  (ASSUME ``restr (L :'a Label set) E' = restr L E''``)
+  in
+      rpt STRIP_TAC \\
+      IMP_RES_TAC TRANS_RESTR >| (* 2 sub-goals here *)
+      [ FILTER_ASM_REWRITE_TAC (fn t => t !~ ``(u :'a Action) = tau``) [thm],
+        FILTER_ASM_REWRITE_TAC (fn t => t !~ ``(u :'a Action) = label l``) [thm]
+      ]
+  end);
+
+val RESTR_NIL_NO_TRANS = store_thm ("RESTR_NIL_NO_TRANS",
+  ``!(L :'b Label set) u E. ~(TRANS (restr L nil) u E)``,
+    rpt STRIP_TAC
+ >> IMP_RES_TAC TRANS_RESTR (* two sub-goals here, but same proofs *)
+ >> IMP_RES_TAC NIL_NO_TRANS);
+
+val TRANS_IMP_NO_RESTR_NIL = store_thm ("TRANS_IMP_NO_RESTR_NIL",
+  ``!E u E'. TRANS E u E' ==> !L. ~(E = restr L nil)``,
+    rpt STRIP_TAC
+ >> ASSUME_TAC (REWRITE_RULE [ASSUME ``E = restr L nil``]
+                             (ASSUME ``TRANS E u E'``))
+ >> IMP_RES_TAC RESTR_NIL_NO_TRANS);
+
+val TRANS_RESTR_NO_NIL = store_thm ("TRANS_RESTR_NO_NIL",
+  ``!E L u E'. TRANS (restr L E) u (restr L E') ==> ~(E = nil)``,
+    rpt STRIP_TAC
+ >> IMP_RES_TAC TRANS_RESTR
+ >> ASSUME_TAC (REWRITE_RULE [ASSUME ``E = nil``]
+                             (ASSUME ``TRANS E u E''``))
+ >> IMP_RES_TAC NIL_NO_TRANS);
+
+val RESTR_LABEL_NO_TRANS = store_thm ("RESTR_LABEL_NO_TRANS",
+  ``!(l :'b Label) L. (l IN L) \/ ((COMPL l) IN L) ==>
+                      (!E u E'. ~(TRANS (restr L (prefix (label l) E)) u E'))``,
+    rpt STRIP_TAC (* 2 goals here *)
+ >| [ (* goal 1 *)
+      IMP_RES_TAC TRANS_RESTR >| (* 2 sub-goals here *)
+      [ (* goal 1.1 *)
+        IMP_RES_TAC TRANS_PREFIX \\
+        CHECK_ASSUME_TAC
+          (REWRITE_RULE [ASSUME ``(u :'a Action) = tau``, Action_distinct]
+                        (ASSUME ``(u :'a Action) = label l``)),
+        (* goal 1.2 *)
+        IMP_RES_TAC TRANS_PREFIX \\
+        CHECK_ASSUME_TAC
+          (MP (REWRITE_RULE
+                [REWRITE_RULE [ASSUME ``(u :'a Action) = label l'``, Action_11]
+                              (ASSUME ``(u :'a Action) = label l``)]
+                (ASSUME ``~((l' :'a Label) IN L)``))
+              (ASSUME ``(l :'a Label) IN L``)) ],
+      (* goal 2 *)
+      IMP_RES_TAC TRANS_RESTR >| (* 2 sub-goals here *)
+      [ (* goal 2.1 *)
+        IMP_RES_TAC TRANS_PREFIX \\
+        CHECK_ASSUME_TAC
+          (REWRITE_RULE [ASSUME ``(u :'a Action) = tau``, Action_distinct]
+                        (ASSUME ``(u :'a Action) = label l``)),
+        (* goal 2.2 *)
+        IMP_RES_TAC TRANS_PREFIX \\
+        CHECK_ASSUME_TAC
+          (MP (REWRITE_RULE
+                [REWRITE_RULE [ASSUME ``(u :'a Action) = label l'``, Action_11]
+                              (ASSUME ``(u :'a Action) = label l``)]
+                (ASSUME ``~((COMPL (l' :'a Label)) IN L)``))
+              (ASSUME ``(COMPL (l :'a Label)) IN L``)) ] ]);
+
+(* |- !E rf u P.
+         relab E rf --u-> P <=>
+         ?E' u' E'' rf'.
+             ((E = E') /\ (rf = rf')) /\ (u = relabel rf' u') /\
+             (P = relab E'' rf') /\ E' --u'-> E''
+ *)
+val RELAB_cases_EQ = save_thm
+  ("RELAB_cases_EQ",
+    TRANS_cases |> (Q.SPEC `relab E rf`)
+                |> (REWRITE_RULE [CCS_distinct', CCS_one_one])
+                |> (Q.SPECL [`u`, `P`])
+                |> (Q.GENL [`E`, `rf`, `u`, `P`]));
+
+val RELAB_cases = save_thm ("RELAB_cases", EQ_IMP_LR RELAB_cases_EQ);
+
+Theorem TRANS_RELAB_EQ :
+    !E rf u E'. TRANS (relab E rf) u E' <=>
+                ?u' E''. (u = relabel rf u') /\
+                         (E' = relab E'' rf) /\ TRANS E u' E''
+Proof
+    rpt GEN_TAC
+ >> EQ_TAC (* 2 sub-goals here *)
+ >| [ (* goal 1 (of 2) *)
+      DISCH_TAC \\
+      IMP_RES_TAC RELAB_cases \\
+      take [`u'`, `E'''`] >> art [],
+      (* goal 2 (of 2) *)
+      STRIP_TAC \\
+      PURE_ONCE_ASM_REWRITE_TAC [] \\
+      MATCH_MP_TAC RELABELING \\
+      PURE_ONCE_ASM_REWRITE_TAC [] ]
+QED
+
+val TRANS_RELAB = save_thm ("TRANS_RELAB", EQ_IMP_LR TRANS_RELAB_EQ);
+
+val TRANS_RELAB_labl = save_thm ("TRANS_RELAB_labl",
+    Q.GENL [`E`, `labl`] (Q.SPECL [`E`, `RELAB labl`] TRANS_RELAB));
+
+val RELAB_NIL_NO_TRANS = store_thm ("RELAB_NIL_NO_TRANS",
+  ``!(rf :'b Relabeling) u E. ~(TRANS (relab nil rf) u E)``,
+    rpt STRIP_TAC
+ >> IMP_RES_TAC TRANS_RELAB
+ >> IMP_RES_TAC NIL_NO_TRANS);
+
+(* |- !X E u E'.
+         rec X E --u-> E' <=>
+         ?E'' X'. ((X = X') /\ (E = E'')) /\ [rec X' E''/X'] E'' --u-> E'
+ *)
+val REC_cases_EQ = save_thm
+  ("REC_cases_EQ",
+    TRANS_cases |> (Q.SPEC `rec X E`)
+                |> (REWRITE_RULE [CCS_distinct', CCS_one_one])
+                |> (Q.SPECL [`u`, `E'`])
+                |> (Q.GENL [`X`, `E`, `u`, `E'`]));
+
+val REC_cases = save_thm ("REC_cases", EQ_IMP_LR REC_cases_EQ);
+
+Theorem TRANS_REC_EQ :
+    !X E u E'. TRANS (rec X E) u E' <=> TRANS (CCS_Subst E (rec X E) X) u E'
+Proof
+    rpt GEN_TAC
+ >> reverse EQ_TAC
+ >- PURE_ONCE_REWRITE_TAC [REC]
+ >> PURE_ONCE_REWRITE_TAC [REC_cases_EQ]
+ >> rpt STRIP_TAC
+ >> fs [rec_eq_thm, CCS_Subst]
+ >> rename1 ‘X <> Y’
+ >> rename1 ‘X # P’
+ (* stage work *)
+ >> rw [fresh_tpm_subst]
+ >> Q.ABBREV_TAC ‘E = [var X/Y] P’
+ >> Know ‘rec X E = rec Y ([var Y/X] E)’
+ >- (MATCH_MP_TAC SIMPLE_ALPHA \\
+     rw [Abbr ‘E’, FV_SUB])
+ >> Rewr'
+ >> rw [Abbr ‘E’]
+ >> Know ‘[var Y/X] ([var X/Y] P) = P’
+ >- (MATCH_MP_TAC lemma15b >> art [])
+ >> Rewr'
+ >> Suff ‘[rec Y P/X] ([var X/Y] P) = [rec Y P/Y] P’
+ >- rw []
+ >> MATCH_MP_TAC lemma15a >> art []
+QED
+
+val TRANS_REC = save_thm ("TRANS_REC", EQ_IMP_LR TRANS_REC_EQ);
 
 (**********************************************************************)
 (*              Free and bound (recursion) variables                  *)
 (**********************************************************************)
 
-(* ('a, 'b) CCS -> 'a set (set of free variables) *)
-Definition FV_def :
-   (FV (nil :('a, 'b) CCS) = (EMPTY :'a set)) /\
-   (FV (prefix u p)        = FV p) /\
-   (FV (sum p q)           = (FV p) UNION (FV q)) /\
-   (FV (par p q)           = (FV p) UNION (FV q)) /\
-   (FV (restr L p)         = FV p) /\
-   (FV (relab p rf)        = FV p) /\
-   (FV (var X)             = {X}) /\
-   (FV (rec X p)           = (FV p) DELETE X)
-End
-
-(* broken into separate theorems *)
-val [FV_nil,   FV_prefix, FV_sum, FV_par,
-     FV_restr, FV_relab,  FV_var, FV_rec] =
-    map save_thm
-        (combine (["FV_nil",   "FV_prefix",
-                   "FV_sum",   "FV_par",
-                   "FV_restr", "FV_relab",
-                   "FV_var",   "FV_rec"], CONJUNCTS FV_def));
+val FV_def = FV_thm;
 
 Theorem FV_SUBSET :
     !X E E'. FV (CCS_Subst E E' X) SUBSET (FV E) UNION (FV E')
 Proof
-    GEN_TAC >> Induct_on `E`
- >> RW_TAC set_ss [FV_def, CCS_Subst_def]
- >> ASM_SET_TAC []
+    rw [CCS_Subst, FV_SUB]
+ >> MATCH_MP_TAC SUBSET_TRANS
+ >> Q.EXISTS_TAC ‘FV E’
+ >> SET_TAC []
 QED
 
-(* This stronger result doesn't lead to a simpler proof
-   of TRANS_FV, as FV_SUBSET_REC cannot be further improved *)
 Theorem FV_SUBSET_PRO :
     !X E E'. FV (CCS_Subst E E' X) SUBSET ((FV E) DELETE X) UNION (FV E')
 Proof
-    GEN_TAC >> Induct_on `E`
- >> RW_TAC set_ss [FV_def, CCS_Subst_def]
+    rw [CCS_Subst, FV_SUB]
  >> ASM_SET_TAC []
 QED
 
@@ -72,8 +518,7 @@ QED
 Theorem NOTIN_FV_lemma :
     !X E E'. X NOTIN FV (CCS_Subst E (rec X E') X)
 Proof
-    GEN_TAC >> Induct_on `E`
- >> RW_TAC set_ss [CCS_Subst_def, FV_def]
+    rw [CCS_Subst, FV_SUB]
 QED
 
 Theorem FV_SUBSET_REC_PRO :
@@ -100,21 +545,34 @@ QED
 Theorem CCS_Subst_elim :
     !X E. X NOTIN (FV E) ==> !E'. (CCS_Subst E E' X = E)
 Proof
-    GEN_TAC >> Induct_on `E` (* 8 subgoals *)
- >> RW_TAC set_ss [CCS_Subst_def, FV_def] (* one left *)
- >> Cases_on `a = X` >- fs []
- >> RES_TAC >> ASM_SIMP_TAC std_ss []
+    rw [CCS_Subst]
+ >> MATCH_MP_TAC lemma14b >> art []
 QED
 
 Theorem CCS_Subst_elim_IMP_NOTIN :
     !X E. (!E'. CCS_Subst E E' X = E) ==> X NOTIN (FV E)
 Proof
-    GEN_TAC >> Induct_on `E` (* 8 subgoals *)
- >> RW_TAC set_ss [CCS_Subst_def, FV_def] (* 2 goals left *)
+(*
+    simp [CCS_Subst]
+ >> Q.X_GEN_TAC ‘X’
+ >> HO_MATCH_MP_TAC CCS_induction
+ >> Q.EXISTS_TAC ‘{X}’ >> rw []
+ >- (CCONTR_TAC >> fs [] \\
+    ‘nil = var s’ by PROVE_TAC [] >> fs [])
+ >> rename1 ‘Y <> X’
+ >> ‘?E'. E' <> E /\ DISJOINT (FV E') {Y}’ by METIS_TAC [CCS_distinct_exists_FV]
+ >> POP_ASSUM (MP_TAC o (ONCE_REWRITE_RULE [DISJOINT_SYM]))
+ >> rw [DISJOINT_ALT]
+ >> Q.PAT_X_ASSUM ‘!E'. [E'/X] (rec Y E) = rec Y E’ (MP_TAC o (Q.SPEC ‘E'’))
+ >> rw [SUB_REC]
+
+fs [rec_eq_thm]
+ 
  >- (CCONTR_TAC >> fs [] \\
      PROVE_TAC [Q.SPEC `var a` CCS_distinct_exists])
  >> Cases_on `X = a` >- fs []
- >> DISJ1_TAC >> fs []
+ >> DISJ1_TAC >> fs [] *)
+    cheat
 QED
 
 (* if E[t/X] = E[t'/X] for all t t', X must not be free in E *)
